moved some lemmas to a separate file

trillium/program_logic/adequacy_wip.v
@@ -5,40 +5,13 @@ From iris.base_logic.lib Require Import wsat later_credits.
 From iris.proofmode Require Import tactics.
 From trillium.prelude Require Import quantifiers iris_extraction finitary classical_instances.
 From trillium.program_logic Require Export weakestpre traces.
+From trillium.program_logic Require Export adequacy_utils.
 
 Set Default Proof Using "Type".
 Import uPred.
 
-(* TODO: move *)
-Lemma step_tp_length {Λ} c c' oζ:
-  locale_step (Λ := Λ) c oζ c' → length c.1 ≤ length c'.1.
-Proof.
-  inversion 1; simplify_eq; last done.
-  rewrite !app_length /= !app_length; lia.
-Qed.
-
-Lemma valid_exec_length {Λ} ex (tp1 tp2 : list $ expr Λ) σ1 σ2:
-  valid_exec ex ->
-  trace_starts_in ex (tp1, σ1) ->
-  trace_ends_in ex (tp2, σ2) ->
-  length tp1 ≤ length tp2.
-Proof.
-    revert σ1 σ2 tp1 tp2. induction ex as [| ex IH oζ c']; intros σ1 σ2 tp1 tp2.
-    - intros ? -> Heq. inversion Heq; simplify_eq; done.
-    - intros Hval Hstarts Hends.
-      inversion Hval as [A B|A [tp' σ'] C D E Hstep]. simplify_eq.
-      etransitivity; first eapply IH =>//.
-      pose proof (step_tp_length _ _ _ Hstep) as Hlen. simpl in *.
-      rewrite ->Hends in Hlen. simpl in Hlen. lia.
-Qed.
-
 Notation wptp_from t0 s t Φs := ([∗ list] tp1_e;Φ ∈ (prefixes_from t0 t);Φs, WP tp1_e.2 @ s; locale_of tp1_e.1 tp1_e.2; ⊤ {{ Φ }})%I.
 Notation wptp s t Φs := (wptp_from [] s t Φs).
-
-Notation posts_of t Φs :=
-  ([∗ list] vΦ ∈
-    (omap (λ x, (λ v, (v, x.2)) <$> to_val x.1)
-          (zip_with (λ x y, (x, y)) t Φs)), vΦ.2 vΦ.1)%I.
 
 Definition config_wp `{!irisG Λ M Σ} : iProp Σ :=
   □ ∀ ex atr c1 σ2 ,
@@ -107,566 +80,8 @@ Proof.
   iExists _, _. iApply "IH"; done.
 Qed.
 
-Notation locales_equiv_from t0 t0' t1 t1' :=
-  (Forall2 (λ '(t, e) '(t', e'), locale_of t e = locale_of t' e')
-           (prefixes_from t0 t1) (prefixes_from t0' t1')).
-
-Section locales_helpers.
-  Context {Λ: language}.
-
-  Lemma locales_equiv_from_app (t0 t0' t1 t1' t2 t2': list (expr Λ)):
-    locales_equiv_from t0 t0' t1 t1' ->
-    locales_equiv_from (t0 ++ t1) (t0' ++ t1') t2 t2' ->
-    locales_equiv_from t0 t0' (t1 ++ t2) (t1' ++ t2').
-  Proof.
-    revert t0 t0' t1 t2 t2'. induction t1' ; intros t0 t0' t1 t2 t2' Hequiv1 Hequiv2.
-    - destruct t1; last by apply Forall2_cons_nil_inv in Hequiv1. simpl.
-      clear Hequiv1. revert t0 t0' t2 Hequiv2; induction t2'; intros t0 t0' t2 Hequiv2.
-      + destruct t2; last by apply Forall2_cons_nil_inv in Hequiv2. constructor.
-      + destruct t2; first by inversion Hequiv2.
-        rewrite !(right_id_L [] (++)) // in Hequiv2.
-    - destruct t1; first by inversion Hequiv1.
-      replace ((e :: t1) ++ t2) with (e :: (t1 ++ t2)); last by list_simplifier.
-      replace ((a :: t1') ++ t2') with (a :: (t1' ++ t2')); last by list_simplifier.
-      simpl. constructor.
-      + inversion Hequiv1 =>//.
-      + apply IHt1'.
-        * inversion Hequiv1 =>//.
-        * by list_simplifier.
-  Qed.
-
-  Lemma prefixes_from_length {A} (t0 t1: list A):
-    length (prefixes_from t0 t1) = length t1.
-  Proof. revert t0; induction t1; intros ?; [done|]; rewrite /= IHt1 //. Qed.
-
-  Lemma locales_equiv_from_impl (t0 t0' t1 t1' t2 t2': list (expr Λ)):
-    length t2 = length t2' ->
-    locales_equiv_from t0 t0' (t1 ++ t2) (t1' ++ t2') ->
-    locales_equiv_from (t0 ++ t1) (t0' ++ t1') t2 t2'.
-  Proof.
-    revert t0 t0' t1 t1' t2. induction t2'; intros t0 t0' t1 t1' t2 Hlen Hequiv.
-    - destruct t2 ; simpl in *; done.
-    - destruct t2; first done.
-      revert e a t0 t0' t1 t2' t2 IHt2' Hlen Hequiv. induction t1'; intros x y t0 t0' t1 t2' t2 IHt2' Hlen Hequiv.
-      + destruct t1; first by simpl; constructor; list_simplifier.
-        apply Forall2_length in Hequiv. rewrite !prefixes_from_length app_length /= in Hequiv.
-        simpl in Hlen. lia.
-      + destruct t1.
-        { apply Forall2_length in Hequiv. rewrite !prefixes_from_length !app_length /= in Hequiv.
-          simpl in Hlen. lia. }
-        assert (H: locales_equiv_from (t0 ++ e :: t1) (t0' ++ a :: t1')
-                    (x :: t2) (y :: t2')).
-        { replace (t0 ++ e :: t1) with ((t0 ++ [e]) ++ t1); last by list_simplifier.
-          replace (t0' ++ a :: t1') with ((t0' ++ [a]) ++ t1'); last by list_simplifier.
-          apply IHt1' =>//.
-          by list_simplifier. }
-        simpl; constructor; [inversion H =>// |].
-        apply IHt2'; first by simpl in Hlen; lia. done.
-  Qed.
-
-  Lemma locales_equiv_from_refl (t0 t0' t: list (expr Λ)):
-    locales_equiv t0 t0' ->
-    locales_equiv_from t0 t0' t t.
-  Proof.
-    revert t0 t0'; induction t; intros t0 t0' H; simpl; constructor =>//.
-    { apply locale_equiv =>//. }
-    apply IHt. apply locales_equiv_from_app =>//. simpl.
-    constructor; [ by apply locale_equiv | done].
-  Qed.
-
-  Lemma locales_equiv_refl (t: list (expr Λ)):
-    locales_equiv t t.
-  Proof. apply locales_equiv_from_refl. constructor. Qed.
-
-  Lemma locales_equiv_snoc t0 t0' (e e' : expr Λ) t1 t1':
-    locales_equiv t0 t0' ->
-    locales_equiv_from t0 t0' t1 t1' ->
-    locale_of (t0 ++ t1) e = locale_of (t0' ++ t1') e' ->
-    locales_equiv_from t0 t0' (t1 ++ [e]) (t1' ++ [e']).
-  Proof.
-    intros ???.
-    apply locales_equiv_from_app =>//.
-    simpl. by constructor.
-  Qed.
-
-  Lemma locales_equiv_snoc_same t0 (e e' : expr Λ) t1:
-    locale_of (t0 ++ t1) e = locale_of (t0 ++ t1) e' ->
-    locales_equiv_from t0 t0 (t1 ++ [e]) (t1 ++ [e']).
-  Proof.
-    intros ?. apply locales_equiv_snoc =>//; apply locales_equiv_from_refl; apply locales_equiv_refl.
-  Qed.
-
-  Lemma locales_equiv_from_middle t0 (e e' : expr Λ) t1 t2:
-    locale_of (t0 ++ t1) e = locale_of (t0 ++ t1) e' ->
-    locales_equiv_from t0 t0 (t1 ++ e :: t2) (t1 ++ e' :: t2).
-  Proof.
-    intros ?.
-    apply locales_equiv_from_app.
-    - apply locales_equiv_from_refl. apply locales_equiv_refl.
-    - simpl. constructor; first done.
-      apply locales_equiv_from_impl =>//=.
-      constructor =>//. apply locales_equiv_from_refl.
-      apply locales_equiv_snoc_same. by list_simplifier.
-  Qed.
-
-  Lemma locales_equiv_middle (e e' : expr Λ) t1 t2:
-    locale_of t1 e = locale_of t1 e' ->
-    locales_equiv (t1 ++ e :: t2) (t1 ++ e' :: t2).
-  Proof.
-    intros ?. apply locales_equiv_from_middle.
-    by list_simplifier.
-  Qed.
-
-  Lemma locale_step_equiv (c c' : cfg Λ) oζ:
-    locale_step c oζ c' ->
-    locales_equiv c.1 (take (length c.1) c'.1).
-  Proof.
-    intros H. inversion H as [? ? e1 ? e2 ? efs t1 t2|]; simplify_eq; simpl.
-    - replace (t1 ++ e2 :: t2 ++ efs) with ((t1 ++ e2 :: t2) ++ efs); last by list_simplifier.
-      replace (length (t1 ++ e1 :: t2)) with (length (t1 ++ e2 :: t2)); last first.
-      { rewrite !app_length //=. }
-      rewrite take_app_length. apply locales_equiv_middle.
-      eapply locale_step_preserve =>//.
-    - rewrite take_ge =>//. apply locales_equiv_refl.
-  Qed.
-
-  Lemma locales_equiv_from_take (t0 t0' t1 t1' : list $ expr Λ) n:
-    locales_equiv_from t0 t0' t1 t1' ->
-    locales_equiv_from t0 t0' (take n t1) (take n t1').
-  Proof.
-    revert t0 t0' t1 t1'. induction n as [|n IHn]; intros t0 t0' t1 t1' Hequiv; first constructor.
-    destruct t1 as [|e1 t1]; destruct t1' as [|e1' t1']; try by inversion Hequiv.
-    simpl. constructor; first by inversion Hequiv.
-    apply IHn. by inversion Hequiv.
-  Qed.
-
-  Lemma locales_equiv_take (t1 t2 : list $ expr Λ) n:
-    locales_equiv t1 t2 ->
-    locales_equiv (take n t1) (take n t2).
-  Proof. apply locales_equiv_from_take. Qed.
-
-  Lemma locales_equiv_from_transitive (s1 s2 s3 t1 t2 t3 : list $ expr Λ):
-    locales_equiv s1 s2 ->
-    locales_equiv s2 s3 ->
-    locales_equiv_from s1 s2 t1 t2 ->
-    locales_equiv_from s2 s3 t2 t3 ->
-    locales_equiv_from s1 s3 t1 t3.
-  Proof.
-    revert s1 s2 s3 t1 t2. induction t3 as [|e3 t3] ; intros s1 s2 s3 t1 t2 Hpref1 Hpref2 Hequiv1 Hequiv2;
-      destruct t2 as [|e2 t2]; try by inversion Hequiv2; simplify_eq.
-    destruct t1 as [|e1 t1]; try by inversion Hequiv1; simplify_eq.
-    simpl; constructor; first by etransitivity; [inversion Hequiv1 | inversion Hequiv2].
-    eapply (IHt3 _ (s2 ++ [e2]) _ _ t2).
-    - inversion Hequiv1; simplify_eq =>//. by apply locales_equiv_snoc =>//.
-    - inversion Hequiv2; simplify_eq =>//. by apply locales_equiv_snoc =>//.
-    - inversion Hequiv1 =>//.
-    - inversion Hequiv2 => //.
-  Qed.
-
-  Lemma locales_equiv_transitive (t1 t2 t3 : list $ expr Λ):
-    locales_equiv t1 t2 ->
-    locales_equiv t2 t3 ->
-    locales_equiv t1 t3.
-  Proof. apply locales_equiv_from_transitive; constructor. Qed.
-
-  Lemma locale_valid_exec ex (tp1 tp2 : list $ expr Λ) σ1 σ2:
-    valid_exec ex ->
-    trace_starts_in ex (tp1, σ1) ->
-    trace_ends_in ex (tp2, σ2) ->
-    locales_equiv tp1 (take (length tp1) tp2).
-  Proof.
-    revert σ1 σ2 tp1 tp2. induction ex as [| ex IH oζ c']; intros σ1 σ2 tp1 tp2.
-    - intros ? -> Heq. inversion Heq; simplify_eq.
-      rewrite take_ge //. apply locales_equiv_refl.
-    - intros Hval Hstarts Hends.
-      inversion Hval as [A B|A [tp' σ'] C D E Hstep]. simplify_eq.
-      eapply locales_equiv_transitive.
-      eapply IH =>//.
-      pose proof (locale_step_equiv _ _ _ Hstep) as Hequiv.
-      rewrite /trace_ends_in /trace_last in Hends.
-      rewrite Hends in Hequiv.
-      apply (locales_equiv_take _ _ (length tp1)) in Hequiv.
-      rewrite take_take in Hequiv.
-      assert (length tp1 ≤ length tp').
-      { eapply (valid_exec_length ex ) =>//. }
-      simpl in Hequiv.
-      replace (length tp1 `min` length tp') with (length tp1) in Hequiv;
-        [done|lia].
-  Qed.
-
-End locales_helpers.
-
-Section from_locale.
-  Context {Λ: language}.
-  Context `{ EqDecision (locale Λ)}.
-
-  Fixpoint from_locale_from tp0 tp ζ :=
-    match tp with
-    | [] => None
-    | e::tp' => if decide (locale_of tp0 e = ζ) then Some e else from_locale_from (tp0 ++ [e]) tp' ζ
-    end.
-
-  Definition from_locale tp ζ := from_locale_from [] tp ζ.
-
-  (* Other possibility is:
-  Definition from_locale tp ζ := list_find (λ '(tp, e), locale_of tp e = ζ) (prefixes tp).*)
-
-  Lemma from_locale_from_Some_app tp0 tp tp' ζ e :
-    from_locale_from tp0 tp ζ = Some e ->
-    from_locale_from tp0 (tp ++ tp') ζ = Some e.
-  Proof.
-    revert tp0 tp'. induction tp as [|e' tp IH]; first by list_simplifier.
-    simpl. intros tp0 tp' Hfl.
-    destruct (decide (locale_of tp0 e' = ζ)) =>//.
-    apply IH =>//.
-  Qed.
-
-  Lemma from_locale_from_is_Some_app tp0 tp tp' ζ :
-    is_Some (from_locale_from tp0 tp ζ) ->
-    is_Some (from_locale_from tp0 (tp ++ tp') ζ).
-  Proof.
-    intros [? HS]. eapply from_locale_from_Some_app in HS. eauto.
-  Qed.
-
-  Lemma from_locale_from_equiv tp0 tp0' tp tp' ζ :
-    locales_equiv tp0 tp0' ->
-    locales_equiv_from tp0 tp0' tp tp' ->
-    is_Some (from_locale_from tp0 tp ζ) ->
-    is_Some (from_locale_from tp0' tp' ζ).
-  Proof.
-    revert tp0 tp0' tp'. induction tp as [|e tp IH]; intros tp0 tp0' tp' Heq0 Heq [eζ Heζ];
-      destruct tp' as [|e' tp']; try by apply Forall2_length in Heq.
-    simpl in *.
-    destruct (decide (locale_of tp0 e' = ζ)).
-    - rewrite decide_True //; eauto. erewrite <-locale_equiv =>//.
-    - rewrite decide_False; last by erewrite <-locale_equiv.
-      apply Forall2_cons_1 in Heq as [Hlocs ?].
-      rewrite decide_False // in Heζ; last by erewrite Hlocs, <-locale_equiv =>//.
-      apply (IH (tp0 ++ [e])); eauto.
-      apply locales_equiv_snoc =>//.
-  Qed.
-
-  Lemma from_locale_step tp1 tp2 ζ oζ σ1 σ2 :
-    locale_step (tp1, σ1) oζ (tp2, σ2) →
-    is_Some(from_locale tp1 ζ) →
-    is_Some(from_locale tp2 ζ).
-  Proof.
-    intros Hstep. inversion Hstep; simplify_eq=>//.
-    intros HiS. replace (t1 ++ e2 :: t2 ++ efs) with ((t1 ++ e2 :: t2) ++ efs);
-                  last by list_simplifier.
-    apply from_locale_from_is_Some_app.
-    eapply from_locale_from_equiv; eauto; [constructor|].
-    apply locales_equiv_from_middle. list_simplifier. by eapply locale_step_preserve.
-  Qed.
-
-  Lemma from_locale_from_Some tp0 tp1 tp e :
-    (tp, e) ∈ prefixes_from tp0 tp1 →
-    from_locale_from tp0 tp1 (locale_of tp e) = Some e.
-  Proof.
-    revert tp0 tp e; induction tp1 as [| e1 tp1 IH]; intros tp0 tp e Hin; first set_solver.
-    apply elem_of_cons in Hin as [Heq|Hin].
-    { simplify_eq. rewrite /= decide_True //. }
-    rewrite /= decide_False; first by apply IH.
-    fold (prefixes_from (A := expr Λ)) in Hin.
-    by eapply locale_injective.
-  Qed.
-
-End from_locale.
-
-(* TODO: Move *)
-Lemma Forall2_eq {A B} (f : A → B) xs ys :
-  Forall2 (λ x y, f x = f y) xs ys ↔ f <$> xs = f <$> ys.
-Proof.
-  split.
-  - revert ys.
-    induction xs as [|x xs IHxs]; intros ys Hforall.
-    { eapply Forall2_nil_inv_l in Hforall. by simplify_eq. }
-    destruct ys as [|y ys].
-    { by apply Forall2_cons_nil_inv in Hforall. }
-    apply Forall2_cons_1 in Hforall as [Hf Hforall]=> /=.
-    f_equiv; [done|by apply IHxs].
-  - revert ys.
-    induction xs as [|x xs IHxs]; intros ys Hf.
-    { rewrite fmap_nil comm in Hf. eapply fmap_nil_inv in Hf. by simplify_eq. }
-    rewrite fmap_cons comm in Hf.
-    apply fmap_cons_inv in Hf as (y & ys' & Hfxy & Hf & ->).
-    apply Forall2_cons. split; [done|by apply IHxs].
-Qed.
-
-Section locales_utils.
-  Context {Λ: language}.
-
-  Definition locales_of_list_from tp0 (tp: list $ expr Λ): list $ locale Λ :=
-    (λ '(t, e), locale_of t e) <$> (prefixes_from tp0 tp).
-  Notation locales_of_list tp := (locales_of_list_from [] tp).
-
-  Lemma locales_of_list_from_cons es' (e : expr Λ) es :
-    locales_of_list_from es' (e :: es) =
-    locale_of es' e :: locales_of_list_from (es' ++ [e]) es.
-  Proof. done. Qed.
-
-  Lemma locales_of_list_equiv (tp0 tp0' tp1 tp2 : list $ expr Λ) :
-    locales_equiv_from tp0 tp0' tp1 tp2 ↔
-    locales_of_list_from tp0 tp1 = locales_of_list_from tp0' tp2.
-  Proof.
-    split; intros Heq.
-    - apply (Forall2_impl _ (λ x y, uncurry locale_of x = uncurry locale_of y))
-        in Heq; [|by intros [] [] HP].
-      by rewrite Forall2_eq in Heq.
-    - apply (Forall2_impl (λ x y, uncurry locale_of x = uncurry locale_of y));
-        [|by intros [] [] HP].
-      by rewrite Forall2_eq.
-  Qed.
-
-  Lemma locales_of_list_step_incl σ1 σ2 oζ tp1 tp2 :
-    locale_step (tp1, σ1) oζ (tp2, σ2) ->
-    locales_of_list tp1 ⊆ locales_of_list tp2.
-  Proof.
-    intros H. inversion H; simplify_eq=>//.
-    replace (t1 ++ e2 :: t2 ++ efs) with ((t1 ++ e2 :: t2) ++ efs); last by list_simplifier.
-    rewrite /locales_of_list_from. rewrite [in X in _ ⊆ X]prefixes_from_app /= fmap_app.
-    assert ((λ '(t, e), locale_of t e) <$> prefixes (t1 ++ e1 :: t2) = (λ '(t, e), locale_of t e) <$> prefixes (t1 ++ e2 :: t2))
-      as ->; last set_solver.
-    apply locales_of_list_equiv, locales_equiv_middle. by eapply locale_step_preserve.
-  Qed.
-
-  Lemma locales_of_list_from_locale_from `{EqDecision (locale Λ)} tp0 tp1 ζ:
-    is_Some (from_locale_from tp0 tp1 ζ) ->
-    ζ ∈ locales_of_list_from tp0 tp1.
-  Proof.
-    revert tp0; induction tp1 as [|e1 tp1 IH]; intros tp0.
-    { simpl. intros H. inversion H. congruence. }
-    simpl. intros [e Hsome]. rewrite /locales_of_list_from /=.
-    destruct (decide (locale_of tp0 e1 = ζ)); simplify_eq; first set_solver.
-    apply elem_of_cons; right. apply IH. eauto.
-  Qed.
-
-  Definition locales_equiv_prefix_from {Λ} (tp0 tp1 tp2 : list $ expr Λ) :=
-    locales_equiv_from tp0 tp0 tp1 (take (length tp1) tp2).
-  Notation locales_equiv_prefix tp1 tp2 := (locales_equiv_prefix_from [] tp1 tp2).
-
-  Lemma locales_equiv_from_length (tp0 tp0' tp1 tp2 : list $ expr Λ) :
-    locales_equiv_from tp0 tp0' tp1 tp2 → length tp1 = length tp2.
-  Proof. intros Heq%Forall2_length. by rewrite !prefixes_from_length in Heq. Qed.
-
-  Lemma locales_equiv_prefix_from_length (tp0 tp1 tp2 : list $ expr Λ) :
-    locales_equiv_prefix_from tp0 tp1 tp2 → length tp1 ≤ length tp2.
-  Proof.
-    rewrite /locales_equiv_prefix_from.
-    intros ->%locales_equiv_from_length.
-    revert tp2. induction tp1; [simpl; lia|].
-    destruct tp2; [done|by apply le_n_S].
-  Qed.
-
-  Lemma locales_equiv_prefix_from_trans (tp0 tp1 tp2 tp3 : list $ expr Λ) :
-    locales_equiv_prefix_from tp0 tp1 tp2 →
-    locales_equiv_prefix_from tp0 tp2 tp3 →
-    locales_equiv_prefix_from tp0 tp1 tp3.
-  Proof.
-    rewrite /locales_equiv_prefix_from. intros.
-    assert (length tp1 ≤ length tp2);
-      [by eapply locales_equiv_prefix_from_length|].
-    eapply locales_equiv_from_transitive;
-      [apply locales_equiv_refl..|done|].
-    assert (length tp1 = length tp1 `min` length tp2) as Heq by lia.
-    rewrite {2}Heq -take_take. by apply locales_equiv_from_take.
-  Qed.
-
-  Lemma locales_equiv_prefix_trans (tp1 tp2 tp3 : list $ expr Λ) :
-    locales_equiv_prefix tp1 tp2 →
-    locales_equiv_prefix tp2 tp3 →
-    locales_equiv_prefix tp1 tp3.
-  Proof. intros. by eapply locales_equiv_prefix_from_trans. Qed.
-
-  Lemma locales_equiv_from_comm (tp0 tp0' tp1 tp2 : list $ expr Λ) :
-    locales_equiv_from tp0 tp0' tp1 tp2 →
-    locales_equiv_from tp0' tp0 tp2 tp1.
-  Proof. by rewrite !locales_of_list_equiv. Qed.
-
-  Lemma locales_equiv_from_locale_of (tp0 tp0' tp1 tp2 tp3 : list $ expr Λ) :
-    locales_equiv tp0 tp0' →
-    locales_equiv_from tp0 tp1 tp2 tp3 ↔
-    locales_equiv_from tp0' tp1 tp2 tp3.
-  Proof.
-    rewrite !locales_of_list_equiv. intros Heq.
-    split.
-    - intros <-.
-      rewrite -locales_of_list_equiv.
-      rewrite -locales_of_list_equiv in Heq.
-      apply locales_equiv_from_refl.
-      by apply locales_equiv_from_comm.
-    - intros <-.
-      rewrite -locales_of_list_equiv.
-      rewrite -locales_of_list_equiv in Heq.
-      by apply locales_equiv_from_refl.
-  Qed.
-
-  Lemma locales_equiv_prefix_from_drop (tp0 tp1 tp2 : list $ expr Λ) :
-    locales_equiv_prefix_from tp0 tp1 tp2 →
-    locales_equiv_from tp0 tp0 tp2 (tp1 ++ (drop (length tp1) tp2)).
-  Proof.
-    revert tp0 tp2.
-    induction tp1 as [|e1 tp1 IHtp1]; intros tp0 tp2 Heq.
-    { by rewrite /locales_equiv_prefix_from !locales_of_list_equiv. }
-    destruct tp2 as [|e2 tp2].
-    { by rewrite /locales_equiv_prefix_from !locales_of_list_equiv
-        /locales_of_list_from in Heq. }
-    rewrite /locales_equiv_prefix_from !locales_of_list_equiv
-      /locales_of_list_from in Heq.
-    rewrite /locales_of_list_from=> /=.
-    inversion Heq as [[Hlocale Htail]].
-    f_equiv; [done|].
-    rewrite /locales_of_list_from in IHtp1.
-    eapply (locales_equiv_from_locale_of _ (tp0 ++ [e1])).
-    { apply locales_equiv_from_app;
-        [by apply locales_equiv_refl|by apply Forall2_cons]. }
-    apply IHtp1, locales_equiv_from_comm.
-    apply (locales_equiv_from_locale_of (tp0 ++ [e1]) (tp0 ++ [e2])).
-    { apply locales_equiv_from_app;
-        [by apply locales_equiv_refl|by apply Forall2_cons]. }
-    apply locales_equiv_from_comm.
-    rewrite /locales_equiv_prefix_from locales_of_list_equiv
-            /locales_of_list_from.
-    by apply Htail.
-  Qed.
-
-  Lemma locales_equiv_from_drop (t0 t1 t2 t2' : list $ expr Λ) :
-    locales_equiv_prefix_from t0 t1 t2 →
-    locales_equiv_prefix_from t0 t1 t2' →
-    locales_equiv_from t0 t0 t2 t2' →
-    locales_equiv_from (t0++t1) (t0++t1) (drop (length t1) t2) (drop (length t1) t2').
-  Proof.
-    intros Hprefix1 Hprefix2 Hequiv.
-    apply locales_equiv_from_impl.
-    { apply Forall2_length in Hequiv. rewrite !prefixes_from_length in Hequiv.
-      by rewrite !skipn_length Hequiv. }
-    apply locales_equiv_prefix_from_drop in Hprefix1.
-    apply locales_equiv_prefix_from_drop in Hprefix2.
-    apply locales_equiv_from_comm in Hprefix1.
-    assert (locales_equiv_from t0 t0 (t1 ++ drop (length t1) t2) t2').
-    { eapply locales_equiv_from_transitive.
-      - apply locales_equiv_refl.
-      - apply locales_equiv_refl.
-      - apply Hprefix1.
-      - apply Hequiv. }
-    assert (locales_equiv_from t0 t0 (t1 ++ drop (length t1) t2) (t1 ++ drop (length t1) t2')).
-    { eapply locales_equiv_from_transitive.
-      - apply locales_equiv_refl.
-      - apply locales_equiv_refl.
-      - apply H.
-      - apply Hprefix2. }
-    done.
-  Qed.
-
-  (* TODO: Find an alternative to this. Used to resolve coercions. *)
-  Lemma fmap_fmap : forall (A B C:Type)(f:A->B)(g:B->C) (l : list A),
-    g <$> (f <$> l) = (fun x => g (f x)) <$> l.
-  Proof. apply map_map. Qed.
-
-  (* TODO: this can likely be removed by redefining [locale_of]
-   to take one argument *)
-  Lemma locales_of_list_from_fork_post `{!irisG Λ M Σ}
-        (xs ys : list ((list $ expr Λ) * (expr Λ))) :
-    (λ '(t,e), locale_of t e) <$> xs =
-    (λ '(t,e), locale_of t e) <$> ys →
-    (λ '(t,e) v, fork_post (locale_of t e) v) <$> xs =
-    (λ '(t,e) v, fork_post (locale_of t e) v) <$> ys.
-  Proof.
-    intros.
-    set f := locale_of.
-    set g := (λ ζ, λ v, flip weakestpre.fork_post v ζ).
-    assert (∀ (xs : list ((list $ expr Λ) * (expr Λ))),
-              g <$> ((λ '(x,y), f x y) <$> xs) =
-              ((λ '(x,y), g (f x y)) <$> xs)) as Hmap.
-    { intros. rewrite fmap_fmap. f_equiv. apply FunExt. by intros []. }
-    rewrite /f /g in Hmap. rewrite -!Hmap. clear Hmap. by f_equiv.
-  Qed.
-
-  Lemma locales_equiv_prefix_from_drop_alt (tp0 tp1 tp2 : list $ expr Λ) :
-    locales_equiv_prefix_from tp0 tp1 tp2 →
-    (λ '(t, e), locale_of t e) <$> prefixes_from (tp0 ++ tp1) (drop (length tp1) tp2) =
-    drop (length tp1) ((λ '(t, e), locale_of t e) <$> prefixes_from tp0 tp2).
-  Proof.
-    revert tp0 tp2.
-    induction tp1; intros tp0 tp2 Hprefix; [by rewrite right_id|].
-    destruct tp2; [done|].
-    rewrite /locales_equiv_prefix_from in Hprefix. simpl in *.
-    apply Forall2_cons in Hprefix as [Hlocale Hprefix].
-    rewrite -IHtp1; last first.
-    { eapply locales_equiv_from_locale_of;
-        [by apply locales_equiv_snoc_same|done]. }
-    rewrite -locales_of_list_equiv.
-    eapply locales_equiv_from_locale_of;
-      [|apply locales_equiv_from_refl, locales_equiv_refl].
-    rewrite -assoc. by eapply locales_equiv_middle.
-  Qed.
-
-  Lemma locales_equiv_prefix_drop_alt (tp0 tp1 : list $ expr Λ) :
-    locales_equiv_prefix tp0 tp1 →
-    (λ '(t, e), locale_of t e) <$> prefixes_from tp0 (drop (length tp0) tp1) =
-    drop (length tp0) ((λ '(t, e), locale_of t e) <$> prefixes tp1).
-  Proof. apply (locales_equiv_prefix_from_drop_alt []). Qed.
-
-End locales_utils.
-Notation locales_of_list tp := (locales_of_list_from [] tp).
-Notation locales_equiv_prefix tp1 tp2 := (locales_equiv_prefix_from [] tp1 tp2).
-
 Section adequacy_helper_lemmas.
   Context `{!irisG Λ M Σ}.
-
-  Lemma wp_take_step s Φ ex atr tp1 e1 tp2 σ1 e2 σ2 efs ζ:
-    valid_exec ex →
-    prim_step e1 σ1 e2 σ2 efs →
-    trace_ends_in ex (tp1 ++ e1 :: tp2, σ1) →
-    locale_of tp1 e1 = ζ ->
-    state_interp ex atr -∗
-    WP e1 @ s; ζ; ⊤ {{ v, Φ v } } ={⊤,∅}=∗ |={∅}▷=>^(S $ trace_length ex)
-                                             |={∅,⊤}=>
-    ∃ δ' ℓ,
-      state_interp (trace_extend ex (Some ζ) (tp1 ++ e2 :: tp2 ++ efs, σ2))
-                   (trace_extend atr ℓ δ') ∗
-      WP e2 @ s; ζ; ⊤ {{ v, Φ v } } ∗
-      ([∗ list] i↦ef ∈ efs,
-        WP ef @ s; locale_of (tp1 ++ e1 :: tp2 ++ take i efs) ef; ⊤
-        {{ v, fork_post (locale_of (tp1 ++ e1 :: tp2 ++ take i efs) ef) v }}).
-  Proof.
-    iIntros (Hex Hstp Hei Hlocale) "HSI Hwp".
-    rewrite wp_unfold /wp_pre.
-    destruct (to_val e1) eqn:He1.
-    { erewrite val_stuck in He1; done. }
-    iMod ("Hwp" $! _ _ ectx_emp with "[//] [] [] HSI") as "[Hs Hwp]";
-      [by rewrite locale_fill|by rewrite ectx_fill_emp|].
-    iDestruct ("Hwp" with "[]") as "Hwp"; first done.
-    iModIntro.
-    iApply (step_fupdN_wand with "[Hwp]"); first by iApply "Hwp".
-    iIntros "Hwp".
-    rewrite !ectx_fill_emp.
-    iMod "Hwp" as (δ' ℓ) "(? & ? & ?)".
-    iModIntro; iExists _, _; iFrame; done.
-  Qed.
-
-  Lemma wp_not_stuck ex atr K tp1 tp2 σ e s Φ ζ :
-    valid_exec ex →
-    trace_ends_in ex (tp1 ++ ectx_fill K e :: tp2, σ) →
-    locale_of tp1 e = ζ ->
-    state_interp ex atr -∗
-    WP e @ s; ζ; ⊤ {{ v, Φ v }} ={⊤}=∗
-    state_interp ex atr ∗
-    WP e @ s; ζ; ⊤ {{ v, Φ v }} ∗
-    ⌜s = NotStuck → not_stuck e (trace_last ex).2⌝.
-  Proof.
-    iIntros (???) "HSI Hwp".
-    rewrite /not_stuck assoc.
-    iApply fupd_plain_keep_r; iFrame.
-    iIntros "[HSI Hwp]".
-    rewrite wp_unfold /wp_pre.
-    destruct (to_val e) eqn:He.
-    - iModIntro; iPureIntro; eauto.
-    - iApply fupd_plain_mask.
-      iMod ("Hwp" with "[] [] [] HSI") as "[Hs Hwp]"; [done| by erewrite locale_fill|done|].
-      erewrite last_eq_trace_ends_in; last done; simpl.
-      iModIntro; destruct s; [iDestruct "Hs" as %?|]; iPureIntro; by eauto.
-  Qed.
 
   Lemma wptp_from_same_locales t0' t0 s tp Φs:
     locales_equiv t0 t0' ->
@@ -717,23 +132,6 @@ Section adequacy_helper_lemmas.
     eapply Forall2_lookup. intros i. destruct (prefixes t0 !! i) as [[??]|]; by constructor.
   Qed.
 
-  Lemma wp_of_val_post e s Φ ζ:
-    WP e @ s; ζ; ⊤ {{ v, Φ v }} ={⊤}=∗
-    from_option (λ v, |~{⊤}~| Φ v) True (to_val e) ∗
-    (from_option (λ v, |~{⊤}~| Φ v) True (to_val e) -∗
-     WP e @ s; ζ; ⊤ {{ v, Φ v }}).
-  Proof.
-    iIntros "Hwp".
-    rewrite wp_unfold /wp_pre.
-    destruct (to_val e) eqn:He; simpl.
-    - iSplitL.
-      + by iIntros "!>!>".
-      + by iIntros "!> Hwp".
-    - iModIntro.
-      iSplit; first by iClear "Hwp".
-      iIntros "_"; done.
-  Qed.
-
   Lemma wptp_app s t0 t1 t0t1 Φs1 t2 Φs2 :
     t0t1 = t0 ++ t1 ->
     wptp_from t0 s t1 Φs1 -∗ wptp_from t0t1 s t2 Φs2 -∗ wptp_from t0 s (t1 ++ t2) (Φs1 ++ Φs2).
@@ -781,61 +179,6 @@ Section adequacy_helper_lemmas.
       iSplitL "Hback"; [iApply "Hback"|iApply "Htback"]; iFrame; done.
   Qed.
 
-  Notation newelems t t' := (drop (length t) t').
-  Notation newposts t t' :=
-    ((λ '(tnew, e), fork_post (locale_of tnew e)) <$>
-        (prefixes_from t (newelems t t'))).
-
-  Lemma newposts_locales_equiv_helper (t0 t0' t1 t1' t : list (expr Λ)):
-    length t1 = length t1' ->
-    locales_equiv t0 t0' ->
-    (λ '(tnew, e0), fork_post (locale_of tnew e0)) <$>
-        (prefixes_from t0 (newelems t1 t)) =
-    (λ '(tnew, e0), fork_post (locale_of tnew e0)) <$>
-        (prefixes_from t0' (newelems t1' t)).
-  Proof.
-    intros Hlen1 H.
-    assert (Hlen2: length t0 = length t0').
-    { apply Forall2_length in H. rewrite !prefixes_from_length // in H. }
-    revert t0 t0' t1 t1' Hlen1 Hlen2 H. induction t; intros t0 t0' t1 t1' Hlen1 Hlen2 H.
-    - rewrite !drop_nil //.
-    - destruct t1; destruct t1' =>//.
-      + simpl; f_equal; first erewrite locale_equiv=> //.
-        specialize (IHt (t0 ++ [a]) (t0' ++ [a]) _ _ Hlen1).
-        simpl in IHt. rewrite !drop_0 in IHt. apply IHt.
-        * rewrite !app_length. lia.
-        * apply locales_equiv_snoc =>//. list_simplifier. apply locale_equiv =>//.
-      + simpl. apply IHt =>//. simpl in Hlen1. lia.
-  Qed.
-
-  Lemma forkposts_locales_equiv (t0 t0' t1 t1' : list (expr Λ)):
-    locales_equiv_from t0 t0' t1 t1' ->
-    (λ '(tnew, e0), fork_post (locale_of tnew e0)) <$>
-        (prefixes_from t0 t1) =
-    (λ '(tnew, e0), fork_post (locale_of tnew e0)) <$>
-        (prefixes_from t0' t1').
-  Proof.
-    intros H.
-    revert t0 t0' t1' H. induction t1; intros t0 t0' t1' H.
-    - destruct t1' =>//. inversion H.
-    - destruct t1' =>//; first inversion H.
-      inversion H; simplify_eq.
-      simpl; f_equal; first by f_equal.
-      by apply IHt1.
-  Qed.
-
-  Lemma newposts_locales_equiv t0 t0' t:
-    locales_equiv t0 t0' ->
-    newposts t0 t = newposts t0' t.
-  Proof.
-    intros H; apply newposts_locales_equiv_helper =>//.
-    eapply Forall2_length in H. rewrite !prefixes_from_length // in H.
-  Qed.
-
-  Lemma newposts_same_empty t:
-    newposts t t = [].
-  Proof. rewrite drop_ge //. Qed.
-
   Lemma new_threads_wptp_from s t efs:
     (([∗ list] i ↦ ef ∈ efs,
       WP ef @ s; locale_of (t ++ take i efs) ef ; ⊤
@@ -845,9 +188,10 @@ Section adequacy_helper_lemmas.
     (* TODO: factorize the two halves *)
     rewrite big_sepL2_alt; iSplit.
     - iIntros "H". iSplit.
-      { rewrite drop_app_length // map_length !prefixes_from_length //. }
+      { rewrite /newposts /newelems. 
+        rewrite drop_app_length // map_length !prefixes_from_length //. }
       iInduction efs as [|ef efs] "IH" forall (t); first done.
-      rewrite /= !drop_app_length //=.
+      rewrite /newposts /newelems. rewrite /= !drop_app_length //=.
       iDestruct "H" as "[H1 H]". rewrite (right_id [] (++)). iFrame.
       replace (map (λ '(tnew, e), fork_post (locale_of tnew e))
                    (prefixes_from (t ++ [ef]) efs))
@@ -857,10 +201,10 @@ Section adequacy_helper_lemmas.
         iIntros "!>" (k e Hin) "H". by list_simplifier.
       + list_simplifier.
         replace (t ++ ef :: efs) with ((t ++ [ef]) ++ efs); last by list_simplifier.
-        rewrite drop_app_length //.
+        rewrite /newposts /newelems. rewrite drop_app_length //.
     - iIntros "[_ H]".
       iInduction efs as [|ef efs] "IH" forall (t); first done.
-      rewrite /= !drop_app_length //=.
+      rewrite /newposts /newelems. rewrite /= !drop_app_length //=.
       iDestruct "H" as "[H1 H]". rewrite (right_id [] (++)). iFrame.
       replace (map (λ '(tnew, e), fork_post (locale_of tnew e))
                    (prefixes_from (t ++ [ef]) efs))
@@ -870,7 +214,7 @@ Section adequacy_helper_lemmas.
         iIntros "!>" (k e Hin) "H". by list_simplifier.
       + list_simplifier.
         replace (t ++ ef :: efs) with ((t ++ [ef]) ++ efs); last by list_simplifier.
-        rewrite drop_app_length //.
+        rewrite /newposts /newelems. rewrite drop_app_length //.
   Qed.
 
   Lemma take_step s Φs ex atr c c' oζ:
@@ -962,49 +306,6 @@ Section adequacy_helper_lemmas.
   Qed.
 
 End adequacy_helper_lemmas.
-
-(** Fixpoint definition of the soundness goal of Trillium *)
-Definition fupd_to_bupd_aux `{invGS_gen hlc Σ}
-           (rec : coPset → iProp Σ) (E1 : coPset) : iProp Σ :=
-  ∀ (P : iProp Σ) E2, ((|={E1,E2}=> rec E2 -∗ P) ==∗ ◇ P).
-
-Definition fupd_to_bupd `{invGS_gen hlc Σ} :=
-  bi_greatest_fixpoint fupd_to_bupd_aux.
-
-Instance fupd_to_bupd_aux_bi_mono `{invGS_gen hlc Σ} :
-  BiMonoPred (fupd_to_bupd_aux).
-Proof.
-  split.
-  - iIntros (Φ Ψ HΦne HΨne) "#H". iIntros (E1) "HE". iIntros (P E2) "HP".
-    iApply "HE"; iMod "HP"; iModIntro. by iIntros; iApply "HP"; iApply "H".
-  - iIntros (Φ HΦne). by intros ??? ->%leibniz_equiv.
-Qed.
-
-Lemma fupd_to_bupd_unfold `{invGS_gen hlc Σ} E :
-  fupd_to_bupd E ≡ fupd_to_bupd_aux fupd_to_bupd E.
-Proof. by rewrite /fupd_to_bupd greatest_fixpoint_unfold. Qed.
-
-Lemma fupd_to_bupd_soundness_no_lc `{!invGpreS Σ} (Q : iProp Σ) :
-  (∀ `{Hinv: !invGS_gen HasNoLc Σ}, fupd_to_bupd ⊤ -∗ Q) → ⊢ |==> Q.
-Proof.
-  iIntros (Hfupd).
-  iMod (@wsat_alloc _ (invGpreS0.(invGpreS_wsat))) as (Hw) "[Hw HE]".
-  iMod (@later_credits.le_upd.lc_alloc _ (invGpreS0.(invGpreS_lc)) 0) as (Hc) "_".
-  set (Hi := InvG HasNoLc _ Hw Hc).
-  iApply (@Hfupd Hi).
-  assert (NonExpansive (λ E, wsat ∗ ownE E)%I).
-  { by intros ??? ->%leibniz_equiv. }
-  iApply (greatest_fixpoint_coiter _ (λ E, wsat ∗ ownE E)%I with "[] [$Hw $HE]").
-  iIntros "!>" (E1) "?".
-  iIntros (P E2) "HP".
-  rewrite fancy_updates.uPred_fupd_unseal /fancy_updates.uPred_fupd_def /=.
-  iMod ("HP" with "[$]") as ">(Hw & HE & HP)".
-  do 2 iModIntro; iApply "HP"; iFrame.
-Qed.
-
-Lemma fupd_to_bupd_soundness_no_lc' `{!invGpreS Σ} (Q : iProp Σ) `{!Plain Q} :
-  (∀ `{Hinv: !invGS_gen HasNoLc Σ}, fupd_to_bupd ⊤ -∗ Q) → ⊢ Q.
-Proof. iIntros; iMod fupd_to_bupd_soundness_no_lc; done. Qed.
 
 
 Definition all_posts `{irisG Λ M Σ} (tp: list (expr Λ)) es
@@ -1257,7 +558,7 @@ Section StrongAdequacyHelpers.
 
   rel_always_holds_with_trace_inv s trace_inv Φs ξ (es, σ) δ -∗
   cur_tr_repr Hinv s es Φs ex atr ={⊤}=∗
-  ▷ ⌜ξ ex atr⌝ ∗
+  ⌜ξ ex atr⌝ ∗
   rel_always_holds_with_trace_inv s trace_inv Φs ξ (es, σ) δ ∗
   cur_tr_repr Hinv s es Φs ex atr ∗
   ⌜ ∀ e, e ∈ (trace_last ex).1 → s = NotStuck → not_stuck e (trace_last ex).2 ⌝.
@@ -1277,14 +578,14 @@ Section StrongAdequacyHelpers.
     iIntros "(Hstep & PRE & _)".
     iDestruct "PRE" as "(HSI & HTI & Htp)".
       
-      iPoseProof (wptp_of_val_post with "Htp") as "Htp".
-      replace stateI with state_interp by done.
-      iMod (pre_step_elim with "HSI Htp") as "[HSI Htp]".
-      iDestruct ("Htp") as "(Hpost & Hback)".
-      
-      iDestruct ("Hstep" with "[] [] [] [] [] [] [] HSI Hpost") as "[_ Hξ]"; eauto.
-      iApply fupd_plain_mask.
-      iMod ("Hξ" with "HTI") as "%"; auto.
+    iPoseProof (wptp_of_val_post with "Htp") as "Htp".
+    replace stateI with state_interp by done.
+    iMod (pre_step_elim with "HSI Htp") as "[HSI Htp]".
+    iDestruct ("Htp") as "(Hpost & Hback)".
+    
+    iDestruct ("Hstep" with "[] [] [] [] [] [] [] HSI Hpost") as "[_ Hξ]"; eauto.
+    iApply fupd_plain_mask.
+    iMod ("Hξ" with "HTI") as "%"; auto.
   Qed.
 
   Lemma get_trace_inv ex atr δ es σ s
@@ -1300,12 +601,16 @@ Section StrongAdequacyHelpers.
     |} : irisG Λ M Σ):
   rel_always_holds_with_trace_inv s trace_inv Φs ξ (es, σ) δ -∗
   stateI ex atr -∗ steps_from_inv ex atr -∗
-  wptp s (trace_last ex).1 (all_posts (trace_last ex).1 es Φs) ={⊤}=∗
-  trace_inv ex atr ∗
+  wptp s (trace_last ex).1 (all_posts (trace_last ex).1 es Φs)
+    (* cur_tr_repr _ s es Φs ex atr *)
+  ={⊤}=∗
+  trace_inv ex atr ∗   
   rel_always_holds_with_trace_inv s trace_inv Φs ξ (es, σ) δ ∗
-  stateI ex atr ∗ 
+  (* cur_tr_repr _ s es Φs ex atr. *)
+  stateI ex atr ∗ (* steps_from_inv ex atr ∗ *)
   wptp s (trace_last ex).1 (all_posts (trace_last ex).1 es Φs).
   Proof using.
+    (* iIntros "Hstep (HSI & HTI & Htp)". *)
     iIntros "Hstep HSI HTI Htp".
     iPoseProof (wptp_of_val_post with "Htp") as "Htp".
     replace stateI with state_interp by done.
@@ -1392,7 +697,7 @@ Section StrongAdequacyHelpers.
     { by eapply valid_system_trace_valid_exec_trace. }
 
     iMod (get_current_facts with "[$] [$]") as "(Hξ & Hstep & PRE & %NSTUCK)".
-    { repeat split; auto. } 
+    { repeat split; auto. }
 
     iDestruct "PRE" as "(HSI & HTI & Htp)".
     replace stateI with state_interp by done.
@@ -1403,12 +708,12 @@ Section StrongAdequacyHelpers.
     iMod (get_trace_inv with "[$] [$] [$] [$]") as "(HTI & Hstep & HSI & Htp)"; eauto.
     { repeat split; auto. }
     
-  iModIntro. 
-  iIntros "HFtB".
-  iNext; iSplit; first done.
-  iDestruct "Hξ" as %Hξ'.
-  iIntros (c oζ c' Hc Hstep).
-
+    iModIntro. 
+    iIntros "HFtB".
+    iNext; iSplit; first done.
+    iDestruct "Hξ" as %Hξ'.
+    iIntros (c oζ c' Hc Hstep).
+  
   opose proof (trace_ends_in_inj ex c (tp, σ1') Hc _).
   { rewrite Hc1. apply trace_ends_in_last. }
 
@@ -1828,250 +1133,4 @@ Proof.
   iSplit; last first.
   { iIntros "?". iApply ("Hstep" with "[] [] [] [] [] [] [] HSI"); eauto. }
   iModIntro; iIntros "[$ ?]"; done.
-Qed.
-
-(** Since the full adequacy statement is quite a mouthful, we prove some more
-intuitive and simpler corollaries. These lemmas are morover stated in terms of
-[rtc erased_step] so one does not have to provide the trace. *)
-Record adequate_multiple {Λ} (s : stuckness) (es : list $ expr Λ) (σ1 : state Λ)
-       (φs : list (val Λ → state Λ → Prop)) : Prop := {
-  adequate_result ex t2 σ2 i v :
-    i < length es →
-    i < length φs →
-    valid_exec ex  →
-    trace_starts_in ex (es, σ1) →
-    trace_ends_in ex (t2, σ2) →
-    t2 !! i ≫= to_val = Some v →
-    from_option (λ φ, φ v σ2) False (φs !! i);
-  adequate_not_stuck ex t2 σ2 e2 :
-    s = NotStuck →
-    valid_exec ex →
-    trace_starts_in ex (es, σ1) →
-    trace_ends_in ex (t2, σ2) →
-    e2 ∈ t2 → not_stuck e2 σ2
-}.
-
-Definition adequate {Λ} (s : stuckness) (e : expr Λ) (σ1 : state Λ)
-    (φ : val Λ → state Λ → Prop) : Prop :=
-  adequate_multiple s [e] σ1 [φ].
-
-Lemma adequate_multiple_alt {Λ} s es σ1 (φs : list (val Λ → state Λ → Prop)) :
-  adequate_multiple s es σ1 φs ↔ ∀ ex t2 σ2,
-      valid_exec ex →
-      trace_starts_in ex (es, σ1) →
-      trace_ends_in ex (t2, σ2) →
-      (∀ i v,
-         i < length es →
-         i < length φs →
-         t2 !! i ≫= to_val = Some v →
-         from_option (λ φ, φ v σ2) False (φs !! i)) ∧
-      (∀ e2, s = NotStuck → e2 ∈ t2 → not_stuck e2 σ2).
-Proof.
-  split.
-  - intros []; naive_solver.
-  - constructor; naive_solver.
-Qed.
-
-Theorem adequate_multiple_tp_safe {Λ} (es : list $ expr Λ) ex t2 σ1 σ2 φs :
-  adequate_multiple NotStuck es σ1 φs →
-  valid_exec ex →
-  trace_starts_in ex (es, σ1) →
-  trace_ends_in ex (t2, σ2) →
-  Forall (λ e, is_Some (to_val e)) t2 ∨ ∃ t3 σ3, step (t2, σ2) (t3, σ3).
-Proof.
-  intros Had ? ? ?.
-  destruct (decide (Forall (λ e, is_Some (to_val e)) t2)) as [|Ht2]; [by left|].
-  apply (not_Forall_Exists _), Exists_exists in Ht2; destruct Ht2 as (e2&?&He2).
-  destruct (adequate_not_stuck NotStuck es σ1 φs Had ex t2 σ2 e2)
-    as [?|(e3&σ3&efs&?)];
-    rewrite ?eq_None_not_Some; auto.
-  { exfalso. eauto. }
-  destruct (elem_of_list_split t2 e2) as (t2'&t2''&->); auto.
-  right; exists (t2' ++ e3 :: t2'' ++ efs), σ3; econstructor; eauto.
-Qed.
-
-Local Definition wp_adequacy_relation Λ M s (φs : list (val Λ → Prop))
-           (ex : execution_trace Λ) (atr : auxiliary_trace M) : Prop :=
-  ∀ c, trace_ends_in ex c →
-       (∀ i v,
-          i < length φs →
-          c.1 !! i ≫= to_val = Some v →
-          from_option (λ φ, φ v) False (φs !! i)) ∧
-       (∀ e2, s = NotStuck → e2 ∈ c.1 → not_stuck e2 c.2).
-
-Local Lemma wp_adequacy_relation_adequacy_multiple {Λ M} s es σ δ φs (ξ : _ -> _ -> Prop):
-  (forall ex aux, ξ ex aux -> wp_adequacy_relation Λ M s φs ex aux) ->
-  continued_simulation
-    ξ
-    (trace_singleton (es, σ))
-    (trace_singleton δ) →
-  adequate_multiple s es σ ((λ φ v _, φ v) <$> φs).
-Proof.
-  intros Himpl Hsm; apply adequate_multiple_alt.
-  intros ex t2 σ2 Hex Hexstr Hexend.
-  eapply simulation_does_continue in Hex as [atr [? Hatr]]; eauto.
-  rewrite -> continued_simulation_unfold in Hatr.
-  destruct Hatr as (Hψ & Hatr).
-  apply Himpl in Hψ.
-  specialize (Hψ (t2, σ2)) as [Hsafe Hstuck]; [done|].
-  split; [|done].
-  intros i v Hlen1 Hlen2 Ht2.
-  rewrite length_fmap in Hlen2.
-  specialize (Hsafe i v Hlen2 Ht2).
-  clear Himpl Ht2 Hsm Hexstr. revert i es Hlen1 Hlen2 Hsafe.
-  induction φs as [|φ φs Hφs]; intros i es Hlen1 Hlen2 Hsafe; [done|].
-  destruct es as [|e es]; [simpl in *;lia|].
-  rewrite fmap_cons. destruct i; [done|]. simpl in *.
-  eapply (Hφs _ es); [lia|lia|done].
-Qed.
-
-Corollary adequacy_multiple_xi Λ M Σ `{!invGpreS Σ} `{EqDecision (mlabel M), EqDecision M}
-        (s: stuckness)
-        (ξ : execution_trace Λ → auxiliary_trace M → Prop)
-        (φs : list (val Λ → Prop))
-        es σ1 δ1 :
-  length es ≥ 1 →
-  rel_finitary ξ →
-  (∀ `{Hinv : !invGS_gen HasNoLc Σ},
-    ⊢ |={⊤}=> ∃
-         (stateI : execution_trace Λ → auxiliary_trace M → iProp Σ)
-         (trace_inv : execution_trace Λ → auxiliary_trace M → iProp Σ)
-         (Φs : list (val Λ → iProp Σ))
-         (fork_post : locale Λ → val Λ → iProp Σ),
-       let _ : irisG Λ M Σ := IrisG _ _ _ Hinv stateI fork_post in
-       ⌜length φs = length Φs⌝ ∗
-       config_wp ∗
-       ([∗ list] Φ;φ ∈ Φs;φs, ∀ v, Φ v -∗ ⌜φ v⌝) ∗
-       stateI (trace_singleton (es, σ1)) (trace_singleton δ1) ∗
-       wptp s es Φs ∗
-       rel_always_holds_with_trace_inv s trace_inv Φs ξ (es,σ1) δ1) →
-  adequate_multiple s es σ1 ((λ φ v _, φ v) <$> φs).
-Proof.
-  pose (ξ' := λ ex aux, ξ ex aux ∧ wp_adequacy_relation Λ M s φs ex aux).
-  intros ?? Hwp; apply (wp_adequacy_relation_adequacy_multiple (M := M) _ _ _ δ1 _ ξ').
-  { by intros ??[??]. }
-  apply (wp_strong_adequacy_multiple_with_trace_inv Λ M Σ s); [done|..].
-  { apply (rel_finitary_impl ξ' ξ) =>//. by intros ??[??]. }
-  iIntros (?) "".
-  iMod Hwp as (stateI post Φs fork_post) "(%Hlen & config_wp & HΦs & HSI & Hwp & H)".
-  iModIntro; iExists _, _, _, _. iFrame "config_wp HSI Hwp".
-  iIntros (ex atr c Hvlt Hexs Hexe Hatre Hψ Hnst Hlocale) "HSI Hposts".
-  iSpecialize ("H" with "[//] [//] [//] [//] [] [//] [//]").
-  - iPureIntro. intros ??????. by eapply Hψ.
-  - iAssert (⌜∀ i v,
-          i < length φs →
-          c.1 !! i ≫= to_val = Some v →
-          from_option (λ φ, φ v) False (φs !! i)⌝)%I
-      as %Hφ.
-    { iIntros (i v Hi HSome).
-      iClear "H HSI".
-      clear Hwp ξ' Hψ.
-      rewrite /cur_posts_multiple. 
-      rewrite big_sepL_omap big_sepL_zip_with.
-      assert (∃ e, c.1 !! i = Some e ∧ to_val e = Some v) as [e [HSome' Hv]].
-      { by apply bind_Some. }
-      iDestruct (big_sepL_lookup with "Hposts") as "Hposts"; [done|].
-      rewrite lookup_app_l; [|lia].
-      assert (∃ φ, φs !! i = Some φ) as [φ Heqφ].
-      { by apply lookup_lt_is_Some_2. }
-      assert (∃ Φ, Φs !! i = Some Φ) as [Φ HeqΦ].
-      { rewrite Hlen in Hi. by apply lookup_lt_is_Some_2. }
-      rewrite HeqΦ Hv /=.
-      iDestruct (big_sepL2_insert_acc with "HΦs") as "[HΦs _]"; [done|done|].
-      iDestruct ("HΦs" with "Hposts") as "Hφ".
-      by rewrite Heqφ. }
-    iDestruct ("H" with "HSI Hposts") as "[? H]". iSplit =>//.
-    iIntros "H1". iMod ("H" with "H1"). iModIntro. iSplit=>//.
-    iIntros (c' Hc').
-    assert (c' = c) as -> by by eapply trace_ends_in_inj. eauto.
-Qed.
-
-Corollary adequacy_xi Λ M Σ `{!invGpreS Σ} `{EqDecision (mlabel M), EqDecision M}
-        (s: stuckness)
-        (ξ : execution_trace Λ → auxiliary_trace M → Prop)
-        (φ : val Λ → Prop)
-        e1 σ1 δ1 :
-  rel_finitary ξ →
-  (∀ `{Hinv : !invGS_gen HasNoLc Σ},
-    ⊢ |={⊤}=> ∃
-         (stateI : execution_trace Λ → auxiliary_trace M → iProp Σ)
-         (trace_inv : execution_trace Λ → auxiliary_trace M → iProp Σ)
-         (Φ : val Λ → iProp Σ)
-         (fork_post : locale Λ → val Λ → iProp Σ),
-       let _ : irisG Λ M Σ := IrisG _ _ _ Hinv stateI fork_post in
-       config_wp ∗
-       (∀ v, Φ v -∗ ⌜φ v⌝) ∗
-       stateI (trace_singleton ([e1], σ1)) (trace_singleton δ1) ∗
-       WP e1 @ s; locale_of [] e1; ⊤ {{ Φ }} ∗
-       rel_always_holds_with_trace_inv s trace_inv [Φ] ξ ([e1],σ1) δ1) →
-  adequate s e1 σ1 (λ v _, φ v).
-Proof.
-  intros Hsc Hwptp.
-  rewrite /adequate.
-  assert ([λ (v : val Λ) (_ : state Λ), φ v] =
-          (λ φ (v : val Λ) (_ : state Λ), φ v) <$> [φ]) as -> by done.
-  eapply adequacy_multiple_xi; [done|done|done|eauto|done|].
-  iIntros (Hinv) "".
-  iMod (Hwptp Hinv) as (stateI trace_inv Φ fork_post) "(Hwpcfg & HΦ & HSI & Hwp & Hstep)".
-  iModIntro.
-  iExists stateI, trace_inv, [Φ], fork_post; iFrame "Hwpcfg HΦ HSI Hwp".
-  iSplit; [done|]. iSplit; [done|]. iSplit; [done|].
-  iIntros (ex atr c ? ? ? ? ? ? ?) "HSI Hposts".
-  iApply ("Hstep" with "[] [] [] [] [] [] [] HSI"); eauto.
-Qed.
-
-Corollary sim_and_adequacy_multiple_xi Λ M Σ `{!invGpreS Σ} `{EqDecision (mlabel M), EqDecision M}
-        (s: stuckness)
-        (ξ : execution_trace Λ → auxiliary_trace M → Prop)
-        (φs : list (val Λ → Prop))
-        es σ1 δ1 :
-  length es ≥ 1 →
-  rel_finitary ξ →
-  (∀ `{Hinv : !invGS_gen HasNoLc Σ},
-    ⊢ |={⊤}=> ∃
-         (stateI : execution_trace Λ → auxiliary_trace M → iProp Σ)
-         (trace_inv : execution_trace Λ → auxiliary_trace M → iProp Σ)
-         (Φs : list (val Λ → iProp Σ))
-         (fork_post : locale Λ → val Λ → iProp Σ),
-       let _ : irisG Λ M Σ := IrisG _ _ _ Hinv stateI fork_post in
-       ⌜length φs = length Φs⌝ ∗
-       config_wp ∗
-       ([∗ list] Φ;φ ∈ Φs;φs, ∀ v, Φ v -∗ ⌜φ v⌝) ∗
-       stateI (trace_singleton (es, σ1)) (trace_singleton δ1) ∗
-       wptp s es Φs ∗
-       rel_always_holds_with_trace_inv s trace_inv Φs ξ (es,σ1) δ1) →
-  (continued_simulation ξ (trace_singleton (es, σ1)) (trace_singleton δ1) ∧
-     adequate_multiple s es σ1 ((λ φ v _, φ v) <$> φs)).
-Proof.
-  intros ?? Hwp. split; eauto using adequacy_multiple_xi.
-  eapply wp_strong_adequacy_multiple_with_trace_inv; [done|done|done|].
-  iIntros (?). iMod Hwp as (? ? ? ?) "(?&?&?&?&?)".
-  iModIntro. iExists _, _, _, _. iFrame.
-Qed.
-
-Corollary sim_and_adequacy_xi Λ M Σ `{!invGpreS Σ} `{EqDecision (mlabel M), EqDecision M}
-        (s: stuckness)
-        (ξ : execution_trace Λ → auxiliary_trace M → Prop)
-        (φ : val Λ → Prop)
-        e1 σ1 δ1 :
-  rel_finitary ξ →
-  (∀ `{Hinv : !invGS_gen HasNoLc Σ},
-    ⊢ |={⊤}=> ∃
-         (stateI : execution_trace Λ → auxiliary_trace M → iProp Σ)
-         (trace_inv : execution_trace Λ → auxiliary_trace M → iProp Σ)
-         (Φ : val Λ → iProp Σ)
-         (fork_post : locale Λ → val Λ → iProp Σ),
-       let _ : irisG Λ M Σ := IrisG _ _ _ Hinv stateI fork_post in
-       config_wp ∗
-       (∀ v, Φ v -∗ ⌜φ v⌝) ∗
-       stateI (trace_singleton ([e1], σ1)) (trace_singleton δ1) ∗
-       WP e1 @ s; locale_of [] e1; ⊤ {{ Φ }} ∗
-       rel_always_holds_with_trace_inv s trace_inv [Φ] ξ ([e1],σ1) δ1) →
-  (continued_simulation ξ (trace_singleton ([e1], σ1)) (trace_singleton δ1) ∧
-     adequate s e1 σ1 (λ v _, φ v)).
-Proof.
-  intros ? Hwp. split; eauto using adequacy_xi.
-  eapply wp_strong_adequacy_with_trace_inv; [done|done|].
-  iIntros (?). iMod Hwp as (? ? ? ?) "(?&?&?&?&?)".
-  iModIntro. iExists _, _, _, _. iFrame.
 Qed.
