trillium/program_logic/adequacy_utils.v
@@ -1,0 +1,729 @@
+From stdpp Require Import finite.
+From iris.algebra Require Import gmap auth agree gset coPset.
+From iris.bi.lib Require Import fixpoint.
+From iris.base_logic.lib Require Import wsat later_credits.
+From iris.proofmode Require Import tactics.
+From trillium.prelude Require Import quantifiers iris_extraction finitary classical_instances.
+From trillium.program_logic Require Export weakestpre traces.
+
+Set Default Proof Using "Type".
+Import uPred.
+
+(* TODO: move *)
+Lemma step_tp_length {Λ} c c' oζ:
+  locale_step (Λ := Λ) c oζ c' → length c.1 ≤ length c'.1.
+Proof.
+  inversion 1; simplify_eq; last done.
+  rewrite !app_length /= !app_length; lia.
+Qed.
+
+Lemma valid_exec_length {Λ} ex (tp1 tp2 : list $ expr Λ) σ1 σ2:
+  valid_exec ex ->
+  trace_starts_in ex (tp1, σ1) ->
+  trace_ends_in ex (tp2, σ2) ->
+  length tp1 ≤ length tp2.
+Proof.
+    revert σ1 σ2 tp1 tp2. induction ex as [| ex IH oζ c']; intros σ1 σ2 tp1 tp2.
+    - intros ? -> Heq. inversion Heq; simplify_eq; done.
+    - intros Hval Hstarts Hends.
+      inversion Hval as [A B|A [tp' σ'] C D E Hstep]. simplify_eq.
+      etransitivity; first eapply IH =>//.
+      pose proof (step_tp_length _ _ _ Hstep) as Hlen. simpl in *.
+      rewrite ->Hends in Hlen. simpl in Hlen. lia.
+Qed.
+
+Notation posts_of t Φs :=
+  ([∗ list] vΦ ∈
+    (omap (λ x, (λ v, (v, x.2)) <$> to_val x.1)
+          (zip_with (λ x y, (x, y)) t Φs)), vΦ.2 vΦ.1)%I.
+
+Notation locales_equiv_from t0 t0' t1 t1' :=
+  (Forall2 (λ '(t, e) '(t', e'), locale_of t e = locale_of t' e')
+           (prefixes_from t0 t1) (prefixes_from t0' t1')).
+
+Section locales_helpers.
+  Context {Λ: language}.
+
+  Lemma locales_equiv_from_app (t0 t0' t1 t1' t2 t2': list (expr Λ)):
+    locales_equiv_from t0 t0' t1 t1' ->
+    locales_equiv_from (t0 ++ t1) (t0' ++ t1') t2 t2' ->
+    locales_equiv_from t0 t0' (t1 ++ t2) (t1' ++ t2').
+  Proof.
+    revert t0 t0' t1 t2 t2'. induction t1' ; intros t0 t0' t1 t2 t2' Hequiv1 Hequiv2.
+    - destruct t1; last by apply Forall2_cons_nil_inv in Hequiv1. simpl.
+      clear Hequiv1. revert t0 t0' t2 Hequiv2; induction t2'; intros t0 t0' t2 Hequiv2.
+      + destruct t2; last by apply Forall2_cons_nil_inv in Hequiv2. constructor.
+      + destruct t2; first by inversion Hequiv2.
+        rewrite !(right_id_L [] (++)) // in Hequiv2.
+    - destruct t1; first by inversion Hequiv1.
+      replace ((e :: t1) ++ t2) with (e :: (t1 ++ t2)); last by list_simplifier.
+      replace ((a :: t1') ++ t2') with (a :: (t1' ++ t2')); last by list_simplifier.
+      simpl. constructor.
+      + inversion Hequiv1 =>//.
+      + apply IHt1'.
+        * inversion Hequiv1 =>//.
+        * by list_simplifier.
+  Qed.
+
+  Lemma prefixes_from_length {A} (t0 t1: list A):
+    length (prefixes_from t0 t1) = length t1.
+  Proof. revert t0; induction t1; intros ?; [done|]; rewrite /= IHt1 //. Qed.
+
+  Lemma locales_equiv_from_impl (t0 t0' t1 t1' t2 t2': list (expr Λ)):
+    length t2 = length t2' ->
+    locales_equiv_from t0 t0' (t1 ++ t2) (t1' ++ t2') ->
+    locales_equiv_from (t0 ++ t1) (t0' ++ t1') t2 t2'.
+  Proof.
+    revert t0 t0' t1 t1' t2. induction t2'; intros t0 t0' t1 t1' t2 Hlen Hequiv.
+    - destruct t2 ; simpl in *; done.
+    - destruct t2; first done.
+      revert e a t0 t0' t1 t2' t2 IHt2' Hlen Hequiv. induction t1'; intros x y t0 t0' t1 t2' t2 IHt2' Hlen Hequiv.
+      + destruct t1; first by simpl; constructor; list_simplifier.
+        apply Forall2_length in Hequiv. rewrite !prefixes_from_length app_length /= in Hequiv.
+        simpl in Hlen. lia.
+      + destruct t1.
+        { apply Forall2_length in Hequiv. rewrite !prefixes_from_length !app_length /= in Hequiv.
+          simpl in Hlen. lia. }
+        assert (H: locales_equiv_from (t0 ++ e :: t1) (t0' ++ a :: t1')
+                    (x :: t2) (y :: t2')).
+        { replace (t0 ++ e :: t1) with ((t0 ++ [e]) ++ t1); last by list_simplifier.
+          replace (t0' ++ a :: t1') with ((t0' ++ [a]) ++ t1'); last by list_simplifier.
+          apply IHt1' =>//.
+          by list_simplifier. }
+        simpl; constructor; [inversion H =>// |].
+        apply IHt2'; first by simpl in Hlen; lia. done.
+  Qed.
+
+  Lemma locales_equiv_from_refl (t0 t0' t: list (expr Λ)):
+    locales_equiv t0 t0' ->
+    locales_equiv_from t0 t0' t t.
+  Proof.
+    revert t0 t0'; induction t; intros t0 t0' H; simpl; constructor =>//.
+    { apply locale_equiv =>//. }
+    apply IHt. apply locales_equiv_from_app =>//. simpl.
+    constructor; [ by apply locale_equiv | done].
+  Qed.
+
+  Lemma locales_equiv_refl (t: list (expr Λ)):
+    locales_equiv t t.
+  Proof. apply locales_equiv_from_refl. constructor. Qed.
+
+  Lemma locales_equiv_snoc t0 t0' (e e' : expr Λ) t1 t1':
+    locales_equiv t0 t0' ->
+    locales_equiv_from t0 t0' t1 t1' ->
+    locale_of (t0 ++ t1) e = locale_of (t0' ++ t1') e' ->
+    locales_equiv_from t0 t0' (t1 ++ [e]) (t1' ++ [e']).
+  Proof.
+    intros ???.
+    apply locales_equiv_from_app =>//.
+    simpl. by constructor.
+  Qed.
+
+  Lemma locales_equiv_snoc_same t0 (e e' : expr Λ) t1:
+    locale_of (t0 ++ t1) e = locale_of (t0 ++ t1) e' ->
+    locales_equiv_from t0 t0 (t1 ++ [e]) (t1 ++ [e']).
+  Proof.
+    intros ?. apply locales_equiv_snoc =>//; apply locales_equiv_from_refl; apply locales_equiv_refl.
+  Qed.
+
+  Lemma locales_equiv_from_middle t0 (e e' : expr Λ) t1 t2:
+    locale_of (t0 ++ t1) e = locale_of (t0 ++ t1) e' ->
+    locales_equiv_from t0 t0 (t1 ++ e :: t2) (t1 ++ e' :: t2).
+  Proof.
+    intros ?.
+    apply locales_equiv_from_app.
+    - apply locales_equiv_from_refl. apply locales_equiv_refl.
+    - simpl. constructor; first done.
+      apply locales_equiv_from_impl =>//=.
+      constructor =>//. apply locales_equiv_from_refl.
+      apply locales_equiv_snoc_same. by list_simplifier.
+  Qed.
+
+  Lemma locales_equiv_middle (e e' : expr Λ) t1 t2:
+    locale_of t1 e = locale_of t1 e' ->
+    locales_equiv (t1 ++ e :: t2) (t1 ++ e' :: t2).
+  Proof.
+    intros ?. apply locales_equiv_from_middle.
+    by list_simplifier.
+  Qed.
+
+  Lemma locale_step_equiv (c c' : cfg Λ) oζ:
+    locale_step c oζ c' ->
+    locales_equiv c.1 (take (length c.1) c'.1).
+  Proof.
+    intros H. inversion H as [? ? e1 ? e2 ? efs t1 t2|]; simplify_eq; simpl.
+    - replace (t1 ++ e2 :: t2 ++ efs) with ((t1 ++ e2 :: t2) ++ efs); last by list_simplifier.
+      replace (length (t1 ++ e1 :: t2)) with (length (t1 ++ e2 :: t2)); last first.
+      { rewrite !app_length //=. }
+      rewrite take_app_length. apply locales_equiv_middle.
+      eapply locale_step_preserve =>//.
+    - rewrite take_ge =>//. apply locales_equiv_refl.
+  Qed.
+
+  Lemma locales_equiv_from_take (t0 t0' t1 t1' : list $ expr Λ) n:
+    locales_equiv_from t0 t0' t1 t1' ->
+    locales_equiv_from t0 t0' (take n t1) (take n t1').
+  Proof.
+    revert t0 t0' t1 t1'. induction n as [|n IHn]; intros t0 t0' t1 t1' Hequiv; first constructor.
+    destruct t1 as [|e1 t1]; destruct t1' as [|e1' t1']; try by inversion Hequiv.
+    simpl. constructor; first by inversion Hequiv.
+    apply IHn. by inversion Hequiv.
+  Qed.
+
+  Lemma locales_equiv_take (t1 t2 : list $ expr Λ) n:
+    locales_equiv t1 t2 ->
+    locales_equiv (take n t1) (take n t2).
+  Proof. apply locales_equiv_from_take. Qed.
+
+  Lemma locales_equiv_from_transitive (s1 s2 s3 t1 t2 t3 : list $ expr Λ):
+    locales_equiv s1 s2 ->
+    locales_equiv s2 s3 ->
+    locales_equiv_from s1 s2 t1 t2 ->
+    locales_equiv_from s2 s3 t2 t3 ->
+    locales_equiv_from s1 s3 t1 t3.
+  Proof.
+    revert s1 s2 s3 t1 t2. induction t3 as [|e3 t3] ; intros s1 s2 s3 t1 t2 Hpref1 Hpref2 Hequiv1 Hequiv2;
+      destruct t2 as [|e2 t2]; try by inversion Hequiv2; simplify_eq.
+    destruct t1 as [|e1 t1]; try by inversion Hequiv1; simplify_eq.
+    simpl; constructor; first by etransitivity; [inversion Hequiv1 | inversion Hequiv2].
+    eapply (IHt3 _ (s2 ++ [e2]) _ _ t2).
+    - inversion Hequiv1; simplify_eq =>//. by apply locales_equiv_snoc =>//.
+    - inversion Hequiv2; simplify_eq =>//. by apply locales_equiv_snoc =>//.
+    - inversion Hequiv1 =>//.
+    - inversion Hequiv2 => //.
+  Qed.
+
+  Lemma locales_equiv_transitive (t1 t2 t3 : list $ expr Λ):
+    locales_equiv t1 t2 ->
+    locales_equiv t2 t3 ->
+    locales_equiv t1 t3.
+  Proof. apply locales_equiv_from_transitive; constructor. Qed.
+
+  Lemma locale_valid_exec ex (tp1 tp2 : list $ expr Λ) σ1 σ2:
+    valid_exec ex ->
+    trace_starts_in ex (tp1, σ1) ->
+    trace_ends_in ex (tp2, σ2) ->
+    locales_equiv tp1 (take (length tp1) tp2).
+  Proof.
+    revert σ1 σ2 tp1 tp2. induction ex as [| ex IH oζ c']; intros σ1 σ2 tp1 tp2.
+    - intros ? -> Heq. inversion Heq; simplify_eq.
+      rewrite take_ge //. apply locales_equiv_refl.
+    - intros Hval Hstarts Hends.
+      inversion Hval as [A B|A [tp' σ'] C D E Hstep]. simplify_eq.
+      eapply locales_equiv_transitive.
+      eapply IH =>//.
+      pose proof (locale_step_equiv _ _ _ Hstep) as Hequiv.
+      rewrite /trace_ends_in /trace_last in Hends.
+      rewrite Hends in Hequiv.
+      apply (locales_equiv_take _ _ (length tp1)) in Hequiv.
+      rewrite take_take in Hequiv.
+      assert (length tp1 ≤ length tp').
+      { eapply (valid_exec_length ex ) =>//. }
+      simpl in Hequiv.
+      replace (length tp1 `min` length tp') with (length tp1) in Hequiv;
+        [done|lia].
+  Qed.
+
+End locales_helpers.
+
+Section from_locale.
+  Context {Λ: language}.
+  Context `{ EqDecision (locale Λ)}.
+
+  Fixpoint from_locale_from tp0 tp ζ :=
+    match tp with
+    | [] => None
+    | e::tp' => if decide (locale_of tp0 e = ζ) then Some e else from_locale_from (tp0 ++ [e]) tp' ζ
+    end.
+
+  Definition from_locale tp ζ := from_locale_from [] tp ζ.
+
+  (* Other possibility is:
+  Definition from_locale tp ζ := list_find (λ '(tp, e), locale_of tp e = ζ) (prefixes tp).*)
+
+  Lemma from_locale_from_Some_app tp0 tp tp' ζ e :
+    from_locale_from tp0 tp ζ = Some e ->
+    from_locale_from tp0 (tp ++ tp') ζ = Some e.
+  Proof.
+    revert tp0 tp'. induction tp as [|e' tp IH]; first by list_simplifier.
+    simpl. intros tp0 tp' Hfl.
+    destruct (decide (locale_of tp0 e' = ζ)) =>//.
+    apply IH =>//.
+  Qed.
+
+  Lemma from_locale_from_is_Some_app tp0 tp tp' ζ :
+    is_Some (from_locale_from tp0 tp ζ) ->
+    is_Some (from_locale_from tp0 (tp ++ tp') ζ).
+  Proof.
+    intros [? HS]. eapply from_locale_from_Some_app in HS. eauto.
+  Qed.
+
+  Lemma from_locale_from_equiv tp0 tp0' tp tp' ζ :
+    locales_equiv tp0 tp0' ->
+    locales_equiv_from tp0 tp0' tp tp' ->
+    is_Some (from_locale_from tp0 tp ζ) ->
+    is_Some (from_locale_from tp0' tp' ζ).
+  Proof.
+    revert tp0 tp0' tp'. induction tp as [|e tp IH]; intros tp0 tp0' tp' Heq0 Heq [eζ Heζ];
+      destruct tp' as [|e' tp']; try by apply Forall2_length in Heq.
+    simpl in *.
+    destruct (decide (locale_of tp0 e' = ζ)).
+    - rewrite decide_True //; eauto. erewrite <-locale_equiv =>//.
+    - rewrite decide_False; last by erewrite <-locale_equiv.
+      apply Forall2_cons_1 in Heq as [Hlocs ?].
+      rewrite decide_False // in Heζ; last by erewrite Hlocs, <-locale_equiv =>//.
+      apply (IH (tp0 ++ [e])); eauto.
+      apply locales_equiv_snoc =>//.
+  Qed.
+
+  Lemma from_locale_step tp1 tp2 ζ oζ σ1 σ2 :
+    locale_step (tp1, σ1) oζ (tp2, σ2) →
+    is_Some(from_locale tp1 ζ) →
+    is_Some(from_locale tp2 ζ).
+  Proof.
+    intros Hstep. inversion Hstep; simplify_eq=>//.
+    intros HiS. replace (t1 ++ e2 :: t2 ++ efs) with ((t1 ++ e2 :: t2) ++ efs);
+                  last by list_simplifier.
+    apply from_locale_from_is_Some_app.
+    eapply from_locale_from_equiv; eauto; [constructor|].
+    apply locales_equiv_from_middle. list_simplifier. by eapply locale_step_preserve.
+  Qed.
+
+  Lemma from_locale_from_Some tp0 tp1 tp e :
+    (tp, e) ∈ prefixes_from tp0 tp1 →
+    from_locale_from tp0 tp1 (locale_of tp e) = Some e.
+  Proof.
+    revert tp0 tp e; induction tp1 as [| e1 tp1 IH]; intros tp0 tp e Hin; first set_solver.
+    apply elem_of_cons in Hin as [Heq|Hin].
+    { simplify_eq. rewrite /= decide_True //. }
+    rewrite /= decide_False; first by apply IH.
+    fold (prefixes_from (A := expr Λ)) in Hin.
+    by eapply locale_injective.
+  Qed.
+
+End from_locale.
+
+(* TODO: Move *)
+Lemma Forall2_eq {A B} (f : A → B) xs ys :
+  Forall2 (λ x y, f x = f y) xs ys ↔ f <$> xs = f <$> ys.
+Proof.
+  split.
+  - revert ys.
+    induction xs as [|x xs IHxs]; intros ys Hforall.
+    { eapply Forall2_nil_inv_l in Hforall. by simplify_eq. }
+    destruct ys as [|y ys].
+    { by apply Forall2_cons_nil_inv in Hforall. }
+    apply Forall2_cons_1 in Hforall as [Hf Hforall]=> /=.
+    f_equiv; [done|by apply IHxs].
+  - revert ys.
+    induction xs as [|x xs IHxs]; intros ys Hf.
+    { rewrite fmap_nil comm in Hf. eapply fmap_nil_inv in Hf. by simplify_eq. }
+    rewrite fmap_cons comm in Hf.
+    apply fmap_cons_inv in Hf as (y & ys' & Hfxy & Hf & ->).
+    apply Forall2_cons. split; [done|by apply IHxs].
+Qed.
+
+Section locales_utils.
+  Context {Λ: language}.
+
+  Definition locales_of_list_from tp0 (tp: list $ expr Λ): list $ locale Λ :=
+    (λ '(t, e), locale_of t e) <$> (prefixes_from tp0 tp).
+  Notation locales_of_list tp := (locales_of_list_from [] tp).
+
+  Lemma locales_of_list_from_cons es' (e : expr Λ) es :
+    locales_of_list_from es' (e :: es) =
+    locale_of es' e :: locales_of_list_from (es' ++ [e]) es.
+  Proof. done. Qed.
+
+  Lemma locales_of_list_equiv (tp0 tp0' tp1 tp2 : list $ expr Λ) :
+    locales_equiv_from tp0 tp0' tp1 tp2 ↔
+    locales_of_list_from tp0 tp1 = locales_of_list_from tp0' tp2.
+  Proof.
+    split; intros Heq.
+    - apply (Forall2_impl _ (λ x y, uncurry locale_of x = uncurry locale_of y))
+        in Heq; [|by intros [] [] HP].
+      by rewrite Forall2_eq in Heq.
+    - apply (Forall2_impl (λ x y, uncurry locale_of x = uncurry locale_of y));
+        [|by intros [] [] HP].
+      by rewrite Forall2_eq.
+  Qed.
+
+  Lemma locales_of_list_step_incl σ1 σ2 oζ tp1 tp2 :
+    locale_step (tp1, σ1) oζ (tp2, σ2) ->
+    locales_of_list tp1 ⊆ locales_of_list tp2.
+  Proof.
+    intros H. inversion H; simplify_eq=>//.
+    replace (t1 ++ e2 :: t2 ++ efs) with ((t1 ++ e2 :: t2) ++ efs); last by list_simplifier.
+    rewrite /locales_of_list_from. rewrite [in X in _ ⊆ X]prefixes_from_app /= fmap_app.
+    assert ((λ '(t, e), locale_of t e) <$> prefixes (t1 ++ e1 :: t2) = (λ '(t, e), locale_of t e) <$> prefixes (t1 ++ e2 :: t2))
+      as ->; last set_solver.
+    apply locales_of_list_equiv, locales_equiv_middle. by eapply locale_step_preserve.
+  Qed.
+
+  Lemma locales_of_list_from_locale_from `{EqDecision (locale Λ)} tp0 tp1 ζ:
+    is_Some (from_locale_from tp0 tp1 ζ) ->
+    ζ ∈ locales_of_list_from tp0 tp1.
+  Proof.
+    revert tp0; induction tp1 as [|e1 tp1 IH]; intros tp0.
+    { simpl. intros H. inversion H. congruence. }
+    simpl. intros [e Hsome]. rewrite /locales_of_list_from /=.
+    destruct (decide (locale_of tp0 e1 = ζ)); simplify_eq; first set_solver.
+    apply elem_of_cons; right. apply IH. eauto.
+  Qed.
+
+  Definition locales_equiv_prefix_from {Λ} (tp0 tp1 tp2 : list $ expr Λ) :=
+    locales_equiv_from tp0 tp0 tp1 (take (length tp1) tp2).
+  Notation locales_equiv_prefix tp1 tp2 := (locales_equiv_prefix_from [] tp1 tp2).
+
+  Lemma locales_equiv_from_length (tp0 tp0' tp1 tp2 : list $ expr Λ) :
+    locales_equiv_from tp0 tp0' tp1 tp2 → length tp1 = length tp2.
+  Proof. intros Heq%Forall2_length. by rewrite !prefixes_from_length in Heq. Qed.
+
+  Lemma locales_equiv_prefix_from_length (tp0 tp1 tp2 : list $ expr Λ) :
+    locales_equiv_prefix_from tp0 tp1 tp2 → length tp1 ≤ length tp2.
+  Proof.
+    rewrite /locales_equiv_prefix_from.
+    intros ->%locales_equiv_from_length.
+    revert tp2. induction tp1; [simpl; lia|].
+    destruct tp2; [done|by apply le_n_S].
+  Qed.
+
+  Lemma locales_equiv_prefix_from_trans (tp0 tp1 tp2 tp3 : list $ expr Λ) :
+    locales_equiv_prefix_from tp0 tp1 tp2 →
+    locales_equiv_prefix_from tp0 tp2 tp3 →
+    locales_equiv_prefix_from tp0 tp1 tp3.
+  Proof.
+    rewrite /locales_equiv_prefix_from. intros.
+    assert (length tp1 ≤ length tp2);
+      [by eapply locales_equiv_prefix_from_length|].
+    eapply locales_equiv_from_transitive;
+      [apply locales_equiv_refl..|done|].
+    assert (length tp1 = length tp1 `min` length tp2) as Heq by lia.
+    rewrite {2}Heq -take_take. by apply locales_equiv_from_take.
+  Qed.
+
+  Lemma locales_equiv_prefix_trans (tp1 tp2 tp3 : list $ expr Λ) :
+    locales_equiv_prefix tp1 tp2 →
+    locales_equiv_prefix tp2 tp3 →
+    locales_equiv_prefix tp1 tp3.
+  Proof. intros. by eapply locales_equiv_prefix_from_trans. Qed.
+
+  Lemma locales_equiv_from_comm (tp0 tp0' tp1 tp2 : list $ expr Λ) :
+    locales_equiv_from tp0 tp0' tp1 tp2 →
+    locales_equiv_from tp0' tp0 tp2 tp1.
+  Proof. by rewrite !locales_of_list_equiv. Qed.
+
+  Lemma locales_equiv_from_locale_of (tp0 tp0' tp1 tp2 tp3 : list $ expr Λ) :
+    locales_equiv tp0 tp0' →
+    locales_equiv_from tp0 tp1 tp2 tp3 ↔
+    locales_equiv_from tp0' tp1 tp2 tp3.
+  Proof.
+    rewrite !locales_of_list_equiv. intros Heq.
+    split.
+    - intros <-.
+      rewrite -locales_of_list_equiv.
+      rewrite -locales_of_list_equiv in Heq.
+      apply locales_equiv_from_refl.
+      by apply locales_equiv_from_comm.
+    - intros <-.
+      rewrite -locales_of_list_equiv.
+      rewrite -locales_of_list_equiv in Heq.
+      by apply locales_equiv_from_refl.
+  Qed.
+
+  Lemma locales_equiv_prefix_from_drop (tp0 tp1 tp2 : list $ expr Λ) :
+    locales_equiv_prefix_from tp0 tp1 tp2 →
+    locales_equiv_from tp0 tp0 tp2 (tp1 ++ (drop (length tp1) tp2)).
+  Proof.
+    revert tp0 tp2.
+    induction tp1 as [|e1 tp1 IHtp1]; intros tp0 tp2 Heq.
+    { by rewrite /locales_equiv_prefix_from !locales_of_list_equiv. }
+    destruct tp2 as [|e2 tp2].
+    { by rewrite /locales_equiv_prefix_from !locales_of_list_equiv
+        /locales_of_list_from in Heq. }
+    rewrite /locales_equiv_prefix_from !locales_of_list_equiv
+      /locales_of_list_from in Heq.
+    rewrite /locales_of_list_from=> /=.
+    inversion Heq as [[Hlocale Htail]].
+    f_equiv; [done|].
+    rewrite /locales_of_list_from in IHtp1.
+    eapply (locales_equiv_from_locale_of _ (tp0 ++ [e1])).
+    { apply locales_equiv_from_app;
+        [by apply locales_equiv_refl|by apply Forall2_cons]. }
+    apply IHtp1, locales_equiv_from_comm.
+    apply (locales_equiv_from_locale_of (tp0 ++ [e1]) (tp0 ++ [e2])).
+    { apply locales_equiv_from_app;
+        [by apply locales_equiv_refl|by apply Forall2_cons]. }
+    apply locales_equiv_from_comm.
+    rewrite /locales_equiv_prefix_from locales_of_list_equiv
+            /locales_of_list_from.
+    by apply Htail.
+  Qed.
+
+  Lemma locales_equiv_from_drop (t0 t1 t2 t2' : list $ expr Λ) :
+    locales_equiv_prefix_from t0 t1 t2 →
+    locales_equiv_prefix_from t0 t1 t2' →
+    locales_equiv_from t0 t0 t2 t2' →
+    locales_equiv_from (t0++t1) (t0++t1) (drop (length t1) t2) (drop (length t1) t2').
+  Proof.
+    intros Hprefix1 Hprefix2 Hequiv.
+    apply locales_equiv_from_impl.
+    { apply Forall2_length in Hequiv. rewrite !prefixes_from_length in Hequiv.
+      by rewrite !skipn_length Hequiv. }
+    apply locales_equiv_prefix_from_drop in Hprefix1.
+    apply locales_equiv_prefix_from_drop in Hprefix2.
+    apply locales_equiv_from_comm in Hprefix1.
+    assert (locales_equiv_from t0 t0 (t1 ++ drop (length t1) t2) t2').
+    { eapply locales_equiv_from_transitive.
+      - apply locales_equiv_refl.
+      - apply locales_equiv_refl.
+      - apply Hprefix1.
+      - apply Hequiv. }
+    assert (locales_equiv_from t0 t0 (t1 ++ drop (length t1) t2) (t1 ++ drop (length t1) t2')).
+    { eapply locales_equiv_from_transitive.
+      - apply locales_equiv_refl.
+      - apply locales_equiv_refl.
+      - apply H.
+      - apply Hprefix2. }
+    done.
+  Qed.
+
+  (* TODO: Find an alternative to this. Used to resolve coercions. *)
+  Lemma fmap_fmap : forall (A B C:Type)(f:A->B)(g:B->C) (l : list A),
+    g <$> (f <$> l) = (fun x => g (f x)) <$> l.
+  Proof. apply map_map. Qed.
+
+  (* TODO: this can likely be removed by redefining [locale_of]
+   to take one argument *)
+  Lemma locales_of_list_from_fork_post `{!irisG Λ M Σ}
+        (xs ys : list ((list $ expr Λ) * (expr Λ))) :
+    (λ '(t,e), locale_of t e) <$> xs =
+    (λ '(t,e), locale_of t e) <$> ys →
+    (λ '(t,e) v, fork_post (locale_of t e) v) <$> xs =
+    (λ '(t,e) v, fork_post (locale_of t e) v) <$> ys.
+  Proof.
+    intros.
+    set f := locale_of.
+    set g := (λ ζ, λ v, flip weakestpre.fork_post v ζ).
+    assert (∀ (xs : list ((list $ expr Λ) * (expr Λ))),
+              g <$> ((λ '(x,y), f x y) <$> xs) =
+              ((λ '(x,y), g (f x y)) <$> xs)) as Hmap.
+    { intros. rewrite fmap_fmap. f_equiv. apply FunExt. by intros []. }
+    rewrite /f /g in Hmap. rewrite -!Hmap. clear Hmap. by f_equiv.
+  Qed.
+
+  Lemma locales_equiv_prefix_from_drop_alt (tp0 tp1 tp2 : list $ expr Λ) :
+    locales_equiv_prefix_from tp0 tp1 tp2 →
+    (λ '(t, e), locale_of t e) <$> prefixes_from (tp0 ++ tp1) (drop (length tp1) tp2) =
+    drop (length tp1) ((λ '(t, e), locale_of t e) <$> prefixes_from tp0 tp2).
+  Proof.
+    revert tp0 tp2.
+    induction tp1; intros tp0 tp2 Hprefix; [by rewrite right_id|].
+    destruct tp2; [done|].
+    rewrite /locales_equiv_prefix_from in Hprefix. simpl in *.
+    apply Forall2_cons in Hprefix as [Hlocale Hprefix].
+    rewrite -IHtp1; last first.
+    { eapply locales_equiv_from_locale_of;
+        [by apply locales_equiv_snoc_same|done]. }
+    rewrite -locales_of_list_equiv.
+    eapply locales_equiv_from_locale_of;
+      [|apply locales_equiv_from_refl, locales_equiv_refl].
+    rewrite -assoc. by eapply locales_equiv_middle.
+  Qed.
+
+  Lemma locales_equiv_prefix_drop_alt (tp0 tp1 : list $ expr Λ) :
+    locales_equiv_prefix tp0 tp1 →
+    (λ '(t, e), locale_of t e) <$> prefixes_from tp0 (drop (length tp0) tp1) =
+    drop (length tp0) ((λ '(t, e), locale_of t e) <$> prefixes tp1).
+  Proof. apply (locales_equiv_prefix_from_drop_alt []). Qed.
+
+End locales_utils.
+Notation locales_of_list tp := (locales_of_list_from [] tp).
+Notation locales_equiv_prefix tp1 tp2 := (locales_equiv_prefix_from [] tp1 tp2).
+
+Section adequacy_helper_lemmas.
+  Context `{!irisG Λ M Σ}.
+
+  Lemma wp_take_step s Φ ex atr tp1 e1 tp2 σ1 e2 σ2 efs ζ:
+    valid_exec ex →
+    prim_step e1 σ1 e2 σ2 efs →
+    trace_ends_in ex (tp1 ++ e1 :: tp2, σ1) →
+    locale_of tp1 e1 = ζ ->
+    state_interp ex atr -∗
+    WP e1 @ s; ζ; ⊤ {{ v, Φ v } } ={⊤,∅}=∗ |={∅}▷=>^(S $ trace_length ex)
+                                             |={∅,⊤}=>
+    ∃ δ' ℓ,
+      state_interp (trace_extend ex (Some ζ) (tp1 ++ e2 :: tp2 ++ efs, σ2))
+                   (trace_extend atr ℓ δ') ∗
+      WP e2 @ s; ζ; ⊤ {{ v, Φ v } } ∗
+      ([∗ list] i↦ef ∈ efs,
+        WP ef @ s; locale_of (tp1 ++ e1 :: tp2 ++ take i efs) ef; ⊤
+        {{ v, fork_post (locale_of (tp1 ++ e1 :: tp2 ++ take i efs) ef) v }}).
+  Proof.
+    iIntros (Hex Hstp Hei Hlocale) "HSI Hwp".
+    rewrite wp_unfold /wp_pre.
+    destruct (to_val e1) eqn:He1.
+    { erewrite val_stuck in He1; done. }
+    iMod ("Hwp" $! _ _ ectx_emp with "[//] [] [] HSI") as "[Hs Hwp]";
+      [by rewrite locale_fill|by rewrite ectx_fill_emp|].
+    iDestruct ("Hwp" with "[]") as "Hwp"; first done.
+    iModIntro.
+    iApply (step_fupdN_wand with "[Hwp]"); first by iApply "Hwp".
+    iIntros "Hwp".
+    rewrite !ectx_fill_emp.
+    iMod "Hwp" as (δ' ℓ) "(? & ? & ?)".
+    iModIntro; iExists _, _; iFrame; done.
+  Qed.
+
+  Lemma wp_not_stuck ex atr K tp1 tp2 σ e s Φ ζ :
+    valid_exec ex →
+    trace_ends_in ex (tp1 ++ ectx_fill K e :: tp2, σ) →
+    locale_of tp1 e = ζ ->
+    state_interp ex atr -∗
+    WP e @ s; ζ; ⊤ {{ v, Φ v }} ={⊤}=∗
+    state_interp ex atr ∗
+    WP e @ s; ζ; ⊤ {{ v, Φ v }} ∗
+    ⌜s = NotStuck → not_stuck e (trace_last ex).2⌝.
+  Proof.
+    iIntros (???) "HSI Hwp".
+    rewrite /not_stuck assoc.
+    iApply fupd_plain_keep_r; iFrame.
+    iIntros "[HSI Hwp]".
+    rewrite wp_unfold /wp_pre.
+    destruct (to_val e) eqn:He.
+    - iModIntro; iPureIntro; eauto.
+    - iApply fupd_plain_mask.
+      iMod ("Hwp" with "[] [] [] HSI") as "[Hs Hwp]"; [done| by erewrite locale_fill|done|].
+      erewrite last_eq_trace_ends_in; last done; simpl.
+      iModIntro; destruct s; [iDestruct "Hs" as %?|]; iPureIntro; by eauto.
+  Qed.
+
+  Lemma wp_of_val_post e s Φ ζ:
+    WP e @ s; ζ; ⊤ {{ v, Φ v }} ={⊤}=∗
+    from_option (λ v, |~{⊤}~| Φ v) True (to_val e) ∗
+    (from_option (λ v, |~{⊤}~| Φ v) True (to_val e) -∗
+     WP e @ s; ζ; ⊤ {{ v, Φ v }}).
+  Proof.
+    iIntros "Hwp".
+    rewrite wp_unfold /wp_pre.
+    destruct (to_val e) eqn:He; simpl.
+    - iSplitL.
+      + by iIntros "!>!>".
+      + by iIntros "!> Hwp".
+    - iModIntro.
+      iSplit; first by iClear "Hwp".
+      iIntros "_"; done.
+  Qed.
+
+  Definition newelems {A: Type} (t t': list A) := (drop (length t) t').
+  Definition newposts t t' :=
+    ((λ '(tnew, e), fork_post (locale_of tnew e)) <$>
+        (prefixes_from t (newelems t t'))).
+
+  Lemma newposts_locales_equiv_helper (t0 t0' t1 t1' t : list (expr Λ)):
+    length t1 = length t1' ->
+    locales_equiv t0 t0' ->
+    (λ '(tnew, e0), fork_post (locale_of tnew e0)) <$>
+        (prefixes_from t0 (newelems t1 t)) =
+    (λ '(tnew, e0), fork_post (locale_of tnew e0)) <$>
+        (prefixes_from t0' (newelems t1' t)).
+  Proof.
+    intros Hlen1 H.
+    assert (Hlen2: length t0 = length t0').
+    { apply Forall2_length in H. rewrite !prefixes_from_length // in H. }
+    revert t0 t0' t1 t1' Hlen1 Hlen2 H. induction t; intros t0 t0' t1 t1' Hlen1 Hlen2 H.
+    - rewrite /newelems. rewrite !drop_nil //.
+    - destruct t1; destruct t1' =>//.
+      + simpl; f_equal; first erewrite locale_equiv=> //.
+        specialize (IHt (t0 ++ [a]) (t0' ++ [a]) _ _ Hlen1).
+        simpl in IHt. rewrite /newelems in IHt. rewrite !drop_0 in IHt. apply IHt.
+        * rewrite !app_length. lia.
+        * apply locales_equiv_snoc =>//. list_simplifier. apply locale_equiv =>//.
+      + simpl. apply IHt =>//. simpl in Hlen1. lia.
+  Qed.
+
+  Lemma forkposts_locales_equiv (t0 t0' t1 t1' : list (expr Λ)):
+    locales_equiv_from t0 t0' t1 t1' ->
+    (λ '(tnew, e0), fork_post (locale_of tnew e0)) <$>
+        (prefixes_from t0 t1) =
+    (λ '(tnew, e0), fork_post (locale_of tnew e0)) <$>
+        (prefixes_from t0' t1').
+  Proof.
+    intros H.
+    revert t0 t0' t1' H. induction t1; intros t0 t0' t1' H.
+    - destruct t1' =>//. inversion H.
+    - destruct t1' =>//; first inversion H.
+      inversion H; simplify_eq.
+      simpl; f_equal; first by f_equal.
+      by apply IHt1.
+  Qed.
+
+  Lemma newposts_locales_equiv t0 t0' t:
+    locales_equiv t0 t0' ->
+    newposts t0 t = newposts t0' t.
+  Proof.
+    intros H; apply newposts_locales_equiv_helper =>//.
+    eapply Forall2_length in H. rewrite !prefixes_from_length // in H.
+  Qed.
+
+  Lemma newposts_same_empty t:
+    newposts t t = [].
+  Proof. rewrite /newposts /newelems. rewrite drop_ge //. Qed.
+
+End adequacy_helper_lemmas.
+
+(** Fixpoint definition of the soundness goal of Trillium *)
+Definition fupd_to_bupd_aux `{invGS_gen hlc Σ}
+           (rec : coPset → iProp Σ) (E1 : coPset) : iProp Σ :=
+  ∀ (P : iProp Σ) E2, ((|={E1,E2}=> rec E2 -∗ P) ==∗ ◇ P).
+
+Definition fupd_to_bupd `{invGS_gen hlc Σ} :=
+  bi_greatest_fixpoint fupd_to_bupd_aux.
+
+Instance fupd_to_bupd_aux_bi_mono `{invGS_gen hlc Σ} :
+  BiMonoPred (fupd_to_bupd_aux).
+Proof.
+  split.
+  - iIntros (Φ Ψ HΦne HΨne) "#H". iIntros (E1) "HE". iIntros (P E2) "HP".
+    iApply "HE"; iMod "HP"; iModIntro. by iIntros; iApply "HP"; iApply "H".
+  - iIntros (Φ HΦne). by intros ??? ->%leibniz_equiv.
+Qed.
+
+Lemma fupd_to_bupd_unfold `{invGS_gen hlc Σ} E :
+  fupd_to_bupd E ≡ fupd_to_bupd_aux fupd_to_bupd E.
+Proof. by rewrite /fupd_to_bupd greatest_fixpoint_unfold. Qed.
+
+Lemma fupd_to_bupd_soundness_no_lc `{!invGpreS Σ} (Q : iProp Σ) :
+  (∀ `{Hinv: !invGS_gen HasNoLc Σ}, fupd_to_bupd ⊤ -∗ Q) → ⊢ |==> Q.
+Proof.
+  iIntros (Hfupd).
+  iMod (@wsat_alloc _ (invGpreS0.(invGpreS_wsat))) as (Hw) "[Hw HE]".
+  iMod (@later_credits.le_upd.lc_alloc _ (invGpreS0.(invGpreS_lc)) 0) as (Hc) "_".
+  set (Hi := InvG HasNoLc _ Hw Hc).
+  iApply (@Hfupd Hi).
+  assert (NonExpansive (λ E, wsat ∗ ownE E)%I).
+  { by intros ??? ->%leibniz_equiv. }
+  iApply (greatest_fixpoint_coiter _ (λ E, wsat ∗ ownE E)%I with "[] [$Hw $HE]").
+  iIntros "!>" (E1) "?".
+  iIntros (P E2) "HP".
+  rewrite fancy_updates.uPred_fupd_unseal /fancy_updates.uPred_fupd_def /=.
+  iMod ("HP" with "[$]") as ">(Hw & HE & HP)".
+  do 2 iModIntro; iApply "HP"; iFrame.
+Qed.
+
+Lemma fupd_to_bupd_soundness_no_lc' `{!invGpreS Σ} (Q : iProp Σ) `{!Plain Q} :
+  (∀ `{Hinv: !invGS_gen HasNoLc Σ}, fupd_to_bupd ⊤ -∗ Q) → ⊢ Q.
+Proof. iIntros; iMod fupd_to_bupd_soundness_no_lc; done. Qed.
+
+
+  Lemma f2b_helper `{invGS_gen HasNoLc Σ} E1 E2 P
+    {PLAIN: Plain P}:
+    fupd_to_bupd E1 -∗ (|={E1, E2}=> fupd_to_bupd E2 -∗ ▷ P) -∗ ▷ P.
+  Proof using.
+    iIntros "FB X".
+    rewrite {1}fupd_to_bupd_unfold. rewrite /fupd_to_bupd_aux.
+    iApply except_0_later.
+    iApply bupd_elim.
+    iApply "FB".
+    done.
+  Qed.
